progress on high adequacy

src/high/recovery_weakestpre.v
@@ -9,10 +9,10 @@ From iris_named_props Require Import named_props.
 From self.program_logic Require Import crash_weakestpre recovery_weakestpre recovery_adequacy.
 
 From self.high Require Import dprop generational_resources wrappers protocol.
-From self Require Import view extra ipm_tactics if_non_zero view_slice solve_view_le.
+From self Require Import view map_extra extra ipm_tactics if_non_zero view_slice solve_view_le.
 From self.base Require Import primitive_laws wpr_lifting.
 From self.high Require Import generational_resources crash_weakestpre.
-From self.high.modalities Require Import or_lost.
+From self.high.modalities Require Import or_lost nextgen.
 From self.nextgen Require Import nextgen_promises.
 
 Set Default Proof Using "Type".
@@ -33,22 +33,22 @@ Definition wpr_pre `{!nvmBaseG Σ Ω, !nvmHighG Σ Ω, !PerennialG Σ} (s : stuc
   (WPC e @ s ; E
     {{ Φ }}
     {{ ∀ σ mj D σ' (HC : crash_prim_step nvm_crash_lang σ σ') ns n, (* The [n] here actually doesn't matter. *)
-      ⎡ state_interp σ n -∗ global_state_interp (Λ := nvm_lang) () ns mj D [] -∗ ▷
+      ⎡ state_interp σ n -∗ global_state_interp (Λ := nvm_lang) () ns mj D [] ={E}=∗
       (* let hG := (nvm_update Σ hG _ Hc1 names) in *)
       (* interp ∗ *)
       ⚡==> (* this is where we want the post crash modality *)
       |={E}=>
-      state_interp σ' 0 ∗
+      ▷ state_interp σ' 0 ∗
       global_state_interp (Λ := nvm_lang) () (step_count_next ns) mj D [] ∗
       validV ∅ ∗
-      (monPred_at (wpr E e_rec e_rec (λ v, Φr v) Φr) (∅, ∅, ∅)) ⎤
+      ▷ (monPred_at (wpr E e_rec e_rec (λ v, Φr v) Φr) (∅, ∅, ∅)) ⎤
     }})%I.
 
 Local Instance wpr_pre_contractive `{!nvmBaseG Σ Ω, !nvmHighG Σ Ω, !PerennialG Σ} s : Contractive (wpr_pre s).
 Proof.
   rewrite /wpr_pre. intros ??? Hwp ?????.
   apply wpc_ne; eauto; first done.
-  do 17 f_equiv.
+  do 23 f_equiv.
   f_contractive.
   repeat f_equiv.
   apply Hwp.
@@ -97,7 +97,7 @@ Proof.
   iIntros "Hσ Hg".
   iSpecialize ("H" with "[//]").
   iSpecialize ("H" $! _ _ with "Hσ Hg").
-  iModIntro. iModIntro.
+  iMod "H". iModIntro. iModIntro.
   iMod "H" as "($ & $ & $ & H)".
   iModIntro.
   iApply ("IH" with "[H] [HΦ]").
@@ -120,37 +120,37 @@ Qed.
 (** If we have a map of points-to predicates prior to a crash and know what view
 we crashed at, then we can get a map of points-to predicates for the new
 heap. *)
-Lemma map_points_to_to_new `{nvmBaseFixedG Σ} logHists store CV (hG hG' : nvmBaseDeltaG) :
-  consistent_cut CV store →
-  crashed_at (hGD := hG') CV -∗
-  base.post_crash_modality.post_crash_mapsto_map store hG hG' -∗
-  ([∗ map] ℓ ↦ hist ∈ logHists, let hG := hG in ℓ ↦h hist) -∗
-  base.post_crash_modality.post_crash_mapsto_map store hG hG' ∗
-  ([∗ map] ℓ ↦ hist ∈ (slice_of_store CV logHists), let hG := hG' in ℓ ↦h hist).
-Proof.
-  iIntros (cut) "#crashed map pts".
-  iAssert (⌜logHists ⊆ store⌝)%I as %sub.
-  { iDestruct "map" as "[impl _]".
-    rewrite map_subseteq_spec.
-    iIntros (ℓ msg look).
-    iApply "impl".
-    iApply (big_sepM_lookup with "pts"). done. }
-  iDestruct (big_sepM_impl_dom_subseteq_with_resource with "map pts []") as "($ & $ & H)".
-  { apply slice_of_store_dom_subset. }
-  iIntros "!>" (ℓ oldHist newHist look1 look2) "map pts".
-  iDestruct (post_crash_modality.post_crash_map_exchange with "map pts") as "[$ pts]".
-  apply slice_of_store_lookup_inv in look2 as (? & ? & ? & ? & ? & ? & ?).
-  2: {
-    eapply valid_slice_mono_l; first done.
-    apply consistent_cut_valid_slice.
-    done. }
-  iDestruct "pts" as (CV') "[crashed' [right | %left]]";
-    iDestruct (crashed_at_agree with "crashed' crashed") as %->;
-    last congruence.
-  iDestruct "right" as (t msg look'' lookm ?) "newPts".
-  simplify_eq.
-  iFrame.
-Qed.
+(* Lemma map_points_to_to_new `{nvmBaseFixedG Σ} logHists store CV (hG hG' : nvmBaseDeltaG) : *)
+(*   consistent_cut CV store → *)
+(*   crashed_at (hGD := hG') CV -∗ *)
+(*   base.post_crash_modality.post_crash_mapsto_map store hG hG' -∗ *)
+(*   ([∗ map] ℓ ↦ hist ∈ logHists, let hG := hG in ℓ ↦h hist) -∗ *)
+(*   base.post_crash_modality.post_crash_mapsto_map store hG hG' ∗ *)
+(*   ([∗ map] ℓ ↦ hist ∈ (slice_of_store CV logHists), let hG := hG' in ℓ ↦h hist). *)
+(* Proof. *)
+(*   iIntros (cut) "#crashed map pts". *)
+(*   iAssert (⌜logHists ⊆ store⌝)%I as %sub. *)
+(*   { iDestruct "map" as "[impl _]". *)
+(*     rewrite map_subseteq_spec. *)
+(*     iIntros (ℓ msg look). *)
+(*     iApply "impl". *)
+(*     iApply (big_sepM_lookup with "pts"). done. } *)
+(*   iDestruct (big_sepM_impl_dom_subseteq_with_resource with "map pts []") as "($ & $ & H)". *)
+(*   { apply slice_of_store_dom_subset. } *)
+(*   iIntros "!>" (ℓ oldHist newHist look1 look2) "map pts". *)
+(*   iDestruct (post_crash_modality.post_crash_map_exchange with "map pts") as "[$ pts]". *)
+(*   apply slice_of_store_lookup_inv in look2 as (? & ? & ? & ? & ? & ? & ?). *)
+(*   2: { *)
+(*     eapply valid_slice_mono_l; first done. *)
+(*     apply consistent_cut_valid_slice. *)
+(*     done. } *)
+(*   iDestruct "pts" as (CV') "[crashed' [right | %left]]"; *)
+(*     iDestruct (crashed_at_agree with "crashed' crashed") as %->; *)
+(*     last congruence. *)
+(*   iDestruct "right" as (t msg look'' lookm ?) "newPts". *)
+(*   simplify_eq. *)
+(*   iFrame. *)
+(* Qed. *)
 
 Lemma view_to_zero_lookup V ℓ x :
   V !! ℓ = Some x → (view_to_zero V) !! ℓ = Some (MaxNat 0).
@@ -158,7 +158,7 @@ Proof.
   intros look. rewrite /view_to_zero. rewrite lookup_fmap. rewrite look. done.
 Qed.
 
-Lemma or_lost_post_crash_full `{nvmBaseFixedG Σ, hG : nvmBaseDeltaG} CV :
+Lemma or_lost_post_crash_full `{nvmHighG} CV :
   crashed_at CV -∗
   persisted (view_to_zero CV) -∗
   ∀ ℓ P, (∀ t, ⌜CV !! ℓ = Some (MaxNat t)⌝ -∗ P t) -∗ or_lost_post_crash ℓ P.
@@ -174,10 +174,8 @@ Proof.
 Qed.
 
 Section wpr.
-  Context `{nvmG Σ}.
-
   (* Computes the new abstract history based on the old history, the crash *)
-(*   view, and the bumpers. *)
+  (*   view, and the bumpers. *)
   Definition new_abs_hist (abs_hists : gmap loc (gmap time positive))
              (offsets : gmap loc nat) (bumpers : gmap loc (positive → option positive))
     : gmap loc (gmap time positive) :=
@@ -340,1536 +338,1526 @@ Section wpr.
 
   (* Given the state interpretations _before_ a crash we reestablish the *)
 (*   interpretations _after_ a crash. *)
-  Lemma nvm_reinit (hGD : nvmDeltaG) n P TV σ σ' (Hinv : invGS Σ) γcrash :
+  (*  (Hinv : invGS Σ)  *)
+  Lemma nvm_reinit `{!nvmBaseG Σ Ω, !nvmHighG Σ Ω, !PerennialG Σ} n σ σ':
     crash_step σ σ' →
-    ⊢ state_interp σ n -∗
-      ((post_crash P) (TV, hGD)) ==∗
-      ∃ (hD' : nvmDeltaG),
-        ⌜ γcrash = get_crash_name hD' ⌝ ∗
-        validV ∅ ∗
-        ▷ interp (nD := hD') ∗
-        nvm_heap_ctx (hG := _) σ' ∗
-        ▷ P (∅, ∅, ∅, hD').
+    state_interp σ n ⊢ |==> ⚡==> |==>
+    validV ∅ ∗
+    (▷ interp) ∗
+    nvm_heap_ctx σ'.
   Proof.
-    iIntros ([store PV CV pIncl cut]).
-    iIntros "[H1 H2] P".
-    iNamed "H1". iNamed "H2".
-
-    (* Our [phys_hist] may contain only a subset of all the locations in *)
-(*     [store]. But, those that are in [phys_hist] agree with what is in *)
-(*     [store]. *)
-    iAssert (⌜ map_zip_with drop_prefix phys_hists offsets ⊆ store  ⌝)%I
-      as %physHistsSubStore.
-    { rewrite map_subseteq_spec.
-      iIntros (ℓ hist look).
-      iDestruct (big_sepM_lookup with "ptsMap") as "pts"; first eassumption.
-      iApply (gen_heap_valid with "Hσ pts"). }
-
-    (* TODO: find a better place *)
-    iAssert (⌜ global_pview ⊑ PV ⌝)%I as "%pviewPV";
-      first by iApply (persisted_auth_included with "Hpers").
-
-    (* We need to first re-create the ghost state for the base *)
-(*     interpretation. *)
-    iMod (nvm_heap_reinit _ _ _ _ _ γcrash with "Hσ Hpers")
-      as (hGD') "(%crEq & valView & baseMap & baseInterp & #persImpl & #pers &
-                            #newCrashedAt)";
-      try done.
-
-    iDestruct (or_lost_post_crash_full with "newCrashedAt pers") as "#orLost".
-
-    iDestruct (big_sepM2_dom with "ordered") as %domHistsEqOrders.
-    iDestruct (big_sepM2_dom with "bumpMono") as %domOrdersEqBumpers.
-    iDestruct (big_sepM2_dom with "bumperSome") as %domHistsEqBumpers.
-    iDestruct (big_sepM2_dom with "predsFullHold") as %domPhysHistsEqAbsHists.
-    iDestruct (big_sepM2_dom with "oldViewsDiscarded") as %offsetDom.
-
-    (* A name for the set of recovered locations. Per the above equalities this *)
-(*     set could be expressed in a number of other ways (for instance by using *)
-(*     [phys_hists] instead of [abs_hists].)*)
-    set (recLocs := dom CV ∩ dom abs_hists).
-
-    set newOffsets := offsets_add offsets CV.
-
-    (* The new offsets is a valid slice of the abstract history. This should *)
-(*     follow from the relationship between [phys_hists] and the points-to *)
-(*     predicates and the fact that [CV] is a valid slice of these. *)
-
-    set (newAbsHists := new_abs_hist abs_hists newOffsets bumpers).
-
-    iMod (full_map_alloc newAbsHists)
-      as (new_abs_history_name) "(hists' & knowHistories & #fragHistories)".
-
-    assert (recLocs = (dom newOffsets)) as domNewOffsets.
-    { rewrite dom_map_zip_with_L.
-      rewrite -offsetDom. rewrite domPhysHistsEqAbsHists. set_solver+. }
-    assert (recLocs = (dom newAbsHists)) as domNewAbsHists.
-    { rewrite new_abs_hist_dom.
-      rewrite -domHistsEqBumpers.
-      rewrite domNewOffsets.
-      set_solver. }
-    (* Allocate new ghost state for the logical histories. *)
-    rewrite /interp.
-
-    (* We freeze/persist the old authorative resource algebra. *)
-    iMod (ghost_map_auth_persist with "allOrders") as "#allOrders".
-    iMod (ghost_map_auth_persist with "offsets") as "#oldOffsets".
-    (* iMod (own_update with "globalPView") as "oldGlobalPView". *)
-    (* { apply auth_update_auth_persist. } *)
-    (* iDestruct "oldGlobalPView" as "#oldGlobalPView". *)
-    iMod (own_update with "atLocs") as "atLocs".
-    { apply auth_update_auth_persist. }
-    iDestruct "atLocs" as "#atLocs".
-    iMod (own_update with "naLocs") as "naLocs".
-    { apply auth_update_auth_persist. }
-    iDestruct "naLocs" as "#naLocs".
-    iMod (own_all_bumpers_persist with "allBumpers") as "#oldBumpers".
-    iMod (own_update with "full_predicates") as "allFullPredicates".
-    { apply auth_update_auth_persist. }
-    iDestruct "allFullPredicates" as "#allFullPredicates".
-    iMod (own_update with "read_predicates") as "allReadPredicates".
-    { apply auth_update_auth_persist. }
-    iDestruct "allReadPredicates" as "#allReadPredicates".
-    iMod (own_update with "pers_predicates") as "allPersPredicates".
-    { apply auth_update_auth_persist. }
-    iDestruct "allPersPredicates" as "#allPersPredicates".
-    (* iDestruct "history" as "[fullHist1 fullHist2]". *)
-    iMod (full_map_persist with "history") as "#oldFullHist".
-    (* iMod (own_update with "fullHist2") as "oldFullHist2". *)
-    (* { apply auth_update_auth_persist. } *)
-    (* iDestruct "oldFullHist2" as "#oldFullHist2". *)
-    (* Ghost state for physical history. *)
-    iMod (own_update with "physHist") as "oldPhysHist".
-    { apply auth_update_auth_persist. }
-    iDestruct "oldPhysHist" as "#oldPhysHist".
-    iMod (ghost_map_auth_persist with "naView") as "#oldNaView".
-
-    (* Some locations may be lost after a crash. For these we need to *)
-(*     forget/throw away the predicate and preorder that was choosen for the *)
-(*     location. *)
-    set newOrders := restrict recLocs orders.
-    iMod (own_all_preorders_gname_alloc newOrders)
-      as (new_orders_name) "[newOrders #fragOrders]".
-
-    iMod (ghost_map_alloc_persistent newOffsets) as
-      (new_offset_name) "[offsets #offsetPts]".
-
-    set new_global_pview := (restrict recLocs (view_to_zero CV)).
-    iMod (own_alloc (● (new_global_pview: viewUR) ⋅ ◯ _))
-      as (new_pview_lb_name) "[globalPView globalPViewPts]".
-    { apply auth_both_valid. split; first done. apply view_valid. }
-    iDestruct "globalPViewPts" as "#globalPViewPts".
-
-    set newFullPreds := restrict recLocs predicates_full.
-    iMod (know_predicates_alloc newFullPreds) as
-      (new_full_predicates_name) "[newFullPreds #newFullPredsFrag]".
-    set newReadPreds := restrict recLocs predicates_read.
-    iMod (know_predicates_alloc newReadPreds) as
-      (new_read_predicates_name) "[newReadPreds #newReadPredsFrag]".
-    set newPersPreds := restrict recLocs predicates_pers.
-    iMod (know_predicates_alloc newPersPreds) as
-      (new_pers_predicates_name) "[newPersPreds #newPersPredsFrag]".
-
-    set newAtLocs := recLocs ∩ at_locs.
-    iMod (own_alloc (● (newAtLocs : gsetUR _) ⋅ ◯ _))
-      as (new_shared_locs_name) "[newAtLocs atLocsFrag]".
-    { apply auth_both_valid. done. }
-    iDestruct "atLocsFrag" as "#atLocsFrag".
-
-    set newNaLocs := recLocs ∩ na_locs.
-    iMod (own_alloc (● (newNaLocs : gsetUR _) ⋅ ◯ _))
-      as (new_exclusive_locs_name) "[newNaLocs naLocsFrag]".
-    { apply auth_both_valid. done. }
-    iDestruct "naLocsFrag" as "#naLocsFrag".
-
-    pose (newNaViews := gset_to_gmap (∅ : view) newNaLocs).
-    iMod (ghost_map_alloc newNaViews) as (new_na_views_name) "[naView naViewPts]".
-
-    iMod (ghost_map_alloc_persistent
-            (default 1%positive <$> slice_hist (MaxNat <$> newOffsets) abs_hists))
-      as (new_crashed_in_name) "[crashedInAuth #crashedInPts]".
-    iMod (ghost_map_auth_persist with "crashedInAuth") as "#crashedInAuth".
-
-    (* Allocate the new map of bumpers. *)
-    set newBumpers := restrict recLocs bumpers.
-    iMod (own_all_bumpers_alloc newBumpers)
-         as (new_bumpers_name) "[newBumpers #bumpersFrag]".
-
-    set newPhysHists :=
-      (λ (hist : gmap _ _), discard_msg_views <$> hist) <$>
-        (drop_all_above newOffsets phys_hists).
-    iMod (auth_map_map_alloc (A := leibnizO _) newPhysHists)
-      as (new_phys_hist_name) "[newPhysHists #newPhysHistFrag]".
-
-    (* We show a few results that will be useful below. *)
-    iAssert (
-      □ ∀ `(AbstractState ST) ℓ (bumper : ST → ST), ⌜ is_Some (CV !! ℓ) ⌝ -∗
-        own_know_bumper (get_bumpers_name hGD) ℓ bumper -∗
-        ⌜ bumpers !! ℓ = Some _ ⌝ ∗
-        own_know_bumper new_bumpers_name ℓ bumper)%I as "#bumperImpl".
-    { iIntros "!>" (???? ℓ bumper (t & cvLook)) "[mono pts]".
-      iFrame "mono".
-      iDestruct (ghost_map_lookup with "oldBumpers pts") as %bumpersLook.
-      iFrame (bumpersLook).
-      iApply (big_sepM_lookup with "bumpersFrag").
-      apply restrict_lookup_Some.
-      split; first done.
-
-      apply elem_of_dom_2 in cvLook.
-      apply elem_of_dom_2 in bumpersLook.
-      apply elem_of_intersection.
-      rewrite domHistsEqBumpers.
-      split; done. }
-
-    iAssert (
-      □ ∀ `(AbstractState ST) ℓ,
-        ⌜ is_Some (CV !! ℓ) ⌝ -∗
-        know_preorder_loc ℓ (abs_state_relation (ST := ST)) -∗
-        ⌜ orders !! ℓ = Some _ ⌝ ∗
-        own_know_preorder_loc new_orders_name ℓ (abs_state_relation (ST := ST)))%I
-      as "#orderImpl".
-    { iIntros "!>" (???? ℓ (t & cvLook)) "order".
-      iDestruct (ghost_map_lookup with "allOrders order") as %ordersLook.
-      iFrame (ordersLook).
-      iApply (big_sepM_lookup with "fragOrders").
-      apply restrict_lookup_Some.
-      split; first done.
-      apply elem_of_dom_2 in cvLook.
-      apply elem_of_dom_2 in ordersLook.
-      rewrite elem_of_intersection.
-      rewrite domHistsEqOrders.
-      split; done. }
-
-    (* The physical and abstract history has the same timestamps for all *)
-(*     locations. We will need this when we apply [valid_slice_transfer] below. *)
-    iAssert (
-      ⌜∀ ℓ h1 h2, phys_hists !! ℓ = Some h1 → abs_hists !! ℓ = Some h2 → dom h1 = dom h2⌝
-    )%I as %physAbsHistTimestamps.
-    { iIntros (?????).
-      iDestruct (big_sepM2_lookup with "predsFullHold") as (??) "(_ & sep)"; try eassumption.
-      iDestruct "sep" as "(_ & sep)".
-      iApply (big_sepM2_dom with "sep"). }
-
-    (* [CV] is a valid slice of the physical and abstract history. *)
-    assert (valid_slice CV (map_zip_with drop_prefix phys_hists offsets))
-      as cvSlicesPhysHists.
-    { apply consistent_cut_valid_slice in cut.
-      eapply valid_slice_mono_l in cut; last apply physHistsSubStore.
-      done. }
-    assert (valid_slice (MaxNat <$> offsets_add offsets CV) abs_hists) as cvSlicesAbsHists.
-    { apply valid_slice_drop_prefix in cvSlicesPhysHists.
-      eapply valid_slice_transfer; done. }
-
-    (* We are done allocating ghost state and can now present a new bundle of *)
-(*     ghost names. *)
-    iModIntro.
-    set (hD' := {|
-      abs_history_name := new_abs_history_name;
-      phys_history_name := new_phys_hist_name;
-      non_atomic_views_gname := new_na_views_name;
-      crashed_in_name := new_crashed_in_name;
-      full_predicates_name := new_full_predicates_name;
-      read_predicates_name := new_read_predicates_name;
-      pers_predicates_name := new_pers_predicates_name;
-      preorders_name := new_orders_name;
-      offset_name := new_offset_name;
-      exclusive_locs_name := new_exclusive_locs_name;
-      shared_locs_name := new_shared_locs_name;
-      bumpers_name := new_bumpers_name;
-      pview_lb_name := new_pview_lb_name;
-    |}).
-    iExists (NvmDeltaG hGD' hD').
-
-    assert (newNaLocs ## newAtLocs) as newLocsDisjoint.
-    { rewrite /newNaLocs /newAtLocs. set_solver+ locsDisjoint. }
-    assert (dom newAbsHists = newNaLocs ∪ newAtLocs) as newHistDomLocs.
-    { rewrite /newAbsHists /newNaLocs /newAtLocs /recLocs.
-      rewrite -domNewAbsHists.
-      rewrite /recLocs.
-      rewrite histDomLocs.
-      set_solver+. }
-    assert (newAbsHists = restrict newNaLocs newAbsHists ∪
-                          restrict newAtLocs newAbsHists) as split.
-    { apply restrict_disjoint_union. done. }
-    iEval (rewrite split) in "knowHistories".
-    rewrite big_sepM_union.
-    2: { apply restrict_disjoint. done. }
-    iDestruct "knowHistories" as "[naHistories atHistories]".
-
-    iFrame "baseInterp".
-    rewrite /nvm_heap_ctx. rewrite /post_crash.
-    iDestruct ("P" $! _ (restrict na_locs abs_hists) bumpers na_views store _
-                with "persImpl baseMap") as "(baseMap & P)".
-    iDestruct
-      (map_points_to_to_new _ _ _ _ hGD'
-         with "newCrashedAt baseMap ptsMap") as "[baseMap ptsMap]"; first done.
-
-    iAssert (
-      post_crash_resource_persistent hGD {| nvm_delta_base := hGD'; nvm_delta_high := hD' |}
-    ) as "#pcResPers".
-    { iSplit.
-      { (* We show that fragments of the histories may survive a crash. *)
-        iModIntro.
-        iIntros (???? ℓ t offset s bumper) "order oldOffset oldBumper frag".
-        iApply "orLost". iIntros (tC look).
-
-        iDestruct "frag" as (encX decEq) "oldFrag".
-
-        iDestruct ("bumperImpl" $! ST with "[//] oldBumper")
-          as "[%bumpersLook newBumper]".
-        iDestruct ("orderImpl" $! ST with "[//] order")
-          as "[%ordersLook newOrder]".
-        iDestruct (ghost_map_lookup with "oldOffsets oldOffset") as %offsetsLook.
-
-        assert (newOffsets !! ℓ = Some (offset + tC)) as newOffsetsLook.
-        { rewrite /newOffsets.
-          apply map_lookup_zip_with_Some.
-          eexists _, (MaxNat _).
-          split_and!; done. }
-
-        assert (ℓ ∈ recLocs).
-        { rewrite /recLocs.
-          rewrite domHistsEqOrders.
-          apply elem_of_intersection.
-          split; apply elem_of_dom; done. }
-
-        iDestruct (big_sepM_lookup _ _ ℓ with "offsetPts") as "offset".
-        { rewrite /newOffsets.
-          apply map_lookup_zip_with_Some.
-          eexists _, (MaxNat _).
-          split_and!; done. }
-
-        iDestruct (full_map_frag_entry with "oldFullHist oldFrag")
-          as %(oldAbsHist & lookH & hLook).
-
-        eassert _ as newHistLook. { apply new_abs_hist_lookup; done. }
-
-        eassert (is_Some (oldAbsHist !! (offset + tC))) as [sOld oldAbsHistLook].
-        { eapply valid_slice_lookup; try done.
-          rewrite lookup_fmap. rewrite /offsets_add.
-          rewrite map_lookup_zip_with.
-          rewrite look. rewrite offsetsLook. simpl.
-          done. }
-
-        (* TODO: Make this a lemma. *)
-        iDestruct (big_sepM2_lookup with "bumperSome")
-          as %bumperSome; [done|done|].
-        eassert _ as applyBumper.
-        { eapply map_Forall_lookup_1.
-          apply bumperSome.
-          apply oldAbsHistLook. }
-        destruct applyBumper as (? & temp).
-        assert _ as encodeBumper by apply temp.
-        apply encode_bumper_Some_decode in temp as (recS & decEq2 & <-).
-
-        assert (is_Some (phys_hists !! ℓ)) as [physHist physHistsLook].
-        { rewrite -elem_of_dom domPhysHistsEqAbsHists elem_of_dom. done. }
-
-        eassert (is_Some (physHist !! _)) as [msg physHistLook].
-        { apply elem_of_dom.
-          erewrite physAbsHistTimestamps; [ | done | done].
-          apply elem_of_dom.
-          done. }
-
-        eassert _ as applyBumper.
-        { eapply map_Forall_lookup_1.
-          apply bumperSome.
-          apply hLook. }
-        destruct applyBumper as (? & temp).
-        assert _ as encodeBumper2 by apply temp.
-        apply encode_bumper_Some_decode in temp as (? & decEq' & <-).
-        simplify_eq.
-
-        iExists _, _.
-
-        iDestruct (big_sepM_lookup with "crashedInPts") as "#crashedIn".
-        { rewrite lookup_fmap.
-          erewrite slice_hist_lookup_Some; try done.
-          rewrite lookup_fmap.
-          erewrite newOffsetsLook.
-          done. }
-
-        iSplit.
-        { iExists sOld. iFrame "crashedIn". iPureIntro. apply decEq2. }
-        iAssert (frag_entry_unenc new_abs_history_name ℓ (offset + tC) (bumper recS))%I as "#frag".
-        { iDestruct (big_sepM_lookup with "fragHistories") as "HI"; try done.
-          iDestruct (big_sepM_lookup with "HI") as "HI2"; try done.
-          { rewrite /new_hist.
-            rewrite lookup_omap.
-            erewrite drop_above_lookup_t.
-            rewrite oldAbsHistLook /=.
-            rewrite encodeBumper.
-            done. }
-          rewrite /know_frag_history_loc.
-          rewrite /frag_entry_unenc.
-          iExists _.
-          iFrame "HI2".
-          rewrite decode_encode. done. }
-        iFrameF "frag".
-
-        iDestruct (auth_map_map_frag_lookup_singleton with "newPhysHistFrag") as "$".
-        { rewrite /newPhysHists. rewrite lookup_fmap. rewrite /drop_all_above.
-          rewrite map_lookup_zip_with.
-          rewrite newOffsetsLook /=. rewrite physHistsLook /=.
-          done. }
-        { rewrite lookup_fmap drop_above_lookup_t physHistLook. done. }
-
-        iIntros ([lt | ->]%Nat.lt_eq_cases).
-        2: { assert (s = recS) as -> by congruence. iFrame "frag". done. }
-
-        iDestruct (big_sepM_lookup with "fragHistories") as "HI"; try done.
-        iDestruct (big_sepM_lookup with "HI") as "HI2"; try done.
-        { rewrite /new_hist.
-          rewrite lookup_omap.
-          erewrite drop_above_lookup_le; last (apply Nat.lt_le_incl; apply lt).
-          rewrite hLook.
-          simpl.
-          rewrite encodeBumper2.
-          done. }
-        iDestruct (big_sepM2_lookup with "ordered") as %incr; try done.
-        iSplitPure.
-        { eapply encode_relation.encode_relation_decode_iff_1; try done.
-          eapply incr; done. }
-        iExists _.
-        iFrame "HI2".
-        rewrite decode_encode.
-        done. }
-
-      (* The preorder implication. We show that the preorders may survive a *)
-(*         crash. *)
-      iSplit.
-      { iModIntro.
-        iIntros (? ? ? ? ?) "order".
-        iApply "orLost". iIntros (t look).
-        iDestruct ("orderImpl" $! ST with "[//] order") as "[_ $]". }
-
-      (* "post_crash_full_pred_impl" - We show that the predicates survives a *)
-(*       crash. *)
-      iSplitL "".
-      { rewrite /post_crash_full_pred_impl.
-        iModIntro.
-        iIntros (??? ℓ ϕ) "oldFullPred".
-        iApply "orLost". iIntros (t look).
-        iDestruct (own_all_preds_pred with "allFullPredicates oldFullPred")
-          as (encPred predsLook) "#equiv".
-        iNext.
-        rewrite /know_pred.
-        iDestruct (predicates_frag_lookup with "newFullPredsFrag") as "newFullPred".
-        { rewrite /newFullPreds.
-          apply restrict_lookup_Some.
-          split; try done.
-          apply elem_of_dom_2 in look.
-          apply elem_of_dom_2 in predsLook.
-          rewrite /recLocs.
-          rewrite domHistsEqBumpers -FullBumperDoms.
-          set_solver+ look predsLook. }
-        rewrite /full_predicates_name. simpl.
-        iApply (
-          internal_eq_rewrite _ _
-            (λ (r : enc_predicateO),
-              own new_full_predicates_name (◯ {[ℓ := pred_to_ra r]})) with "equiv");
-          last done.
-        solve_proper. }
-      (* "post_crash_read_pred_impl" - We show that the predicates survives a *)
-(*       crash. *)
-      iSplitL "".
-      { rewrite /post_crash_read_pred_impl.
-        iModIntro.
-        iIntros (??? ℓ ϕ) "oldReadPred".
-        iApply "orLost". iIntros (t look).
-        iDestruct (own_all_preds_pred with "allReadPredicates oldReadPred")
-          as (encPred predsLook) "#equiv".
-        iNext.
-        rewrite /know_pred.
-        iDestruct (predicates_frag_lookup with "newReadPredsFrag") as "newReadPred".
-        { rewrite /newReadPreds.
-          apply restrict_lookup_Some.
-          split; try done.
-          apply elem_of_dom_2 in look.
-          apply elem_of_dom_2 in predsLook.
-          rewrite /recLocs.
-          rewrite domHistsEqBumpers -ReadBumperDoms.
-          set_solver+ look predsLook. }
-        rewrite /read_predicates_name. simpl.
-        iApply (
-          internal_eq_rewrite _ _
-            (λ (r : enc_predicateO),
-              own new_read_predicates_name (◯ {[ℓ := pred_to_ra r]})) with "equiv");
-          last done.
-        solve_proper. }
-      (* "post_crash_pers_pred_impl" - We show that the predicates survives a *)
-(*       crash. *)
-      iSplitL "".
-      { rewrite /post_crash_pers_pred_impl.
-        iModIntro.
-        iIntros (??? ℓ ϕ) "oldPersPred".
-        iApply "orLost". iIntros (t look).
-        iDestruct (own_all_preds_pred with "allPersPredicates oldPersPred")
-          as (encPred predsLook) "#equiv".
-        iNext.
-        rewrite /know_pred.
-        iDestruct (predicates_frag_lookup with "newPersPredsFrag") as "newPersPred".
-        { rewrite /newPersPreds.
-          apply restrict_lookup_Some.
-          split; try done.
-          apply elem_of_dom_2 in look.
-          apply elem_of_dom_2 in predsLook.
-          rewrite /recLocs.
-          rewrite domHistsEqBumpers -PersBumperDoms.
-          set_solver+ look predsLook. }
-        rewrite /pers_predicates_name. simpl.
-        iApply (
-          internal_eq_rewrite _ _
-            (λ (r : enc_predicateO),
-              own new_pers_predicates_name (◯ {[ℓ := pred_to_ra r]})) with "equiv");
-          last done.
-        solve_proper. }
-      (* "post_crash_at_loc_impl" - Shared locations. *)
-      iSplit. {
-        rewrite /post_crash_at_loc_impl.
-        iIntros "!>" (ℓ) "sh".
-        iApply "orLost". iIntros (t look).
-        iDestruct (own_valid_2 with "atLocs sh")
-          as %[_ [elem _]]%auth_both_dfrac_valid_discrete.
-        iApply (own_mono with "atLocsFrag").
-        exists (◯ newAtLocs).
-        rewrite -auth_frag_op.
-        rewrite gset_op.
-        f_equiv.
-        apply gset_included in elem.
-        symmetry.
-        eapply subseteq_union_1.
-        rewrite /newAtLocs.
-        apply elem_of_subseteq_singleton.
-        apply elem_of_intersection.
-        split; last set_solver.
-        rewrite /newAbsHists.
-        apply elem_of_intersection.
-        split; last first.
-        { rewrite histDomLocs. set_solver+ elem. }
-        apply elem_of_dom.
-        naive_solver. }
-      iSplit. {
-        rewrite /post_crash_na_loc_impl.
-        iIntros "!>" (ℓ) "sh".
-        iApply "orLost". iIntros (t look).
-        iDestruct (own_valid_2 with "naLocs sh")
-          as %[_ [elem _]]%auth_both_dfrac_valid_discrete.
-        iApply (own_mono with "naLocsFrag").
-        exists (◯ newNaLocs).
-        rewrite -auth_frag_op.
-        rewrite gset_op.
-        f_equiv.
-        apply gset_included in elem.
-        symmetry.
-        eapply subseteq_union_1.
-        rewrite /newNaLocs.
-        apply elem_of_subseteq_singleton.
-        apply elem_of_intersection.
-        split; last set_solver + elem.
-        apply elem_of_dom_2 in look.
-        set_solver+ look histDomLocs elem. }
-      (* "post_crash_offsets_impl" *)
-      iSplit. {
-        rewrite /offsets_impl.
-        iIntros "!>" (ℓ oldOffset) "oldOffset".
-        iApply "orLost". iIntros (t cvLook).
-        iDestruct (ghost_map_lookup with "oldOffsets oldOffset") as %look.
-        iApply (big_sepM_lookup with "offsetPts").
-        rewrite /newOffsets.
-        apply map_lookup_zip_with_Some.
-        eexists _, (MaxNat _).
-        split; first reflexivity.
-        split; done. }
-      (* "post_crash_bumper_impl" *)
-      { iIntros "!>" (? ? ? ? ℓ bumper) "oldBumper".
-        iApply "orLost". iIntros (t cvLook).
-        iDestruct ("bumperImpl" $! ST with "[//] oldBumper")
-          as "[%bumpersLook newBumper]".
-        iFrame "newBumper". } }
-
-    (* We show the assumption for the post crash modality. *)
-    iDestruct ("P" with "[atLocsHistories naHistories naViewPts]") as "[$ pcRes]".
-    { rewrite /post_crash_resource.
-      iFrame "pcResPers".
-      (* "post_crash_na_view_map" *)
-      iSplitL "naViewPts".
-      { rewrite /post_crash_na_view_map.
-        iSplitL "".
-        { iIntros (ℓ q SV). iApply (ghost_map_lookup with "oldNaView"). }
-        iDestruct (big_sepM_impl_strong with "naViewPts []") as "[$ H]".
-        iIntros "!>" (ℓ V).
-        destruct (newNaViews !! ℓ) as [newV|] eqn:eq.
-        - iIntros "newPts look".
-          rewrite /newNaViews in eq.
-          apply lookup_gset_to_gmap_Some in eq as [hup <-].
-          iApply soft_disj_intro_r.
-          iApply "orLost". iIntros (t look).
-          iApply "newPts".
-        - iIntros "_ %naViewsLook".
-          iApply soft_disj_intro_r.
-          iExists _. iFrame "newCrashedAt".
-          iRight. iPureIntro.
-          move: eq.
-          rewrite /newNaViews.
-          rewrite lookup_gset_to_gmap_None.
-          rewrite /newNaLocs.
-          rewrite not_elem_of_intersection.
-          intros [elem|elem].
-          2: { exfalso. apply elem. rewrite -naViewsDom. eapply elem_of_dom_2.
-               apply naViewsLook. }
-          rewrite /recLocs in elem.
-          apply not_elem_of_dom.
-          apply elem_of_dom_2 in naViewsLook.
-          rewrite histDomLocs in elem.
-          rewrite naViewsDom in naViewsLook.
-          set_solver+ elem naViewsLook. }
-      (* "post_crash_full_history_map" *)
-      rewrite /post_crash_full_history_map.
-      iSplitL "atLocsHistories".
-      { iIntros (ℓ q hist) "hist".
-        iDestruct (full_map_full_entry with "oldFullHist hist") as %look.
-        destruct (decide (ℓ ∈ at_locs)) as [?|notElem].
-        { iDestruct (big_sepM_lookup with "atLocsHistories") as "H".
-          { apply restrict_lookup_Some; done. }
-          iCombine "H hist" as "H2".
-          iDestruct (full_entry_valid with "H2") as %val.
-          iPureIntro. exfalso.
-          apply (Qp.not_add_le_l 1 q).
-          apply val. }
-        iPureIntro.
-        apply restrict_lookup_Some.
-        split; first done.
-        apply elem_of_dom_2 in look.
-        set_solver+ notElem histDomLocs look. }
-      iSplitL "".
-      { iIntros (ℓ bumper). iApply (ghost_map_lookup with "oldBumpers"). }
-      iDestruct (big_sepM_impl_strong with "naHistories []") as "[$ H]".
-      iIntros "!>" (ℓ oldAbsHist) "pts".
-      iIntros ([absHistLook elem]%restrict_lookup_Some).
-      assert (is_Some (bumpers !! ℓ)) as [bumper ?].
-      { apply elem_of_dom.
-        rewrite -domHistsEqBumpers.
-        apply elem_of_dom.
-        eexists _. apply absHistLook. }
-      assert (is_Some (offsets !! ℓ)) as [offset ?].
-      { apply elem_of_dom.
-        rewrite -offsetDom domPhysHistsEqAbsHists.
-        apply elem_of_dom.
-        eexists _. apply absHistLook. }
-      assert (is_Some (phys_hists !! ℓ)) as [physHist physHistsLook].
-      { rewrite -elem_of_dom domPhysHistsEqAbsHists elem_of_dom. done. }
-      iExists bumper. iSplitPure; first done.
-      iApply soft_disj_intro_r.
-      iApply "orLost". iIntros (tC cvLook).
-      assert (newOffsets !! ℓ = Some (offset + tC)) as newOffsetsLook.
-      { rewrite /newOffsets.
-        apply map_lookup_zip_with_Some.
-        eexists _, (MaxNat _).
-        split_and!; done. }
-
-      rewrite restrict_lookup_elem_of.
-      2: { rewrite /newNaLocs.
-        apply elem_of_dom_2 in cvLook.
-        apply elem_of_dom_2 in absHistLook.
-        set_solver+ elem cvLook absHistLook. }
-      eassert (new_abs_hist abs_hists newOffsets bumpers !! ℓ = Some _)
-        as newAbsHistLook.
-      { apply map_lookup_zip_with_Some.
-        eexists _, _.
-        split_and!; try done.
-        rewrite /drop_all_above.
-        apply map_lookup_zip_with_Some.
-        eexists _, _.
-        split_and!; done. }
-      rewrite newAbsHistLook.
-      eassert (is_Some (oldAbsHist !! (offset + tC))) as [sOld ?].
-      { eapply valid_slice_lookup; try done.
-        rewrite lookup_fmap. rewrite /offsets_add.
-        rewrite map_lookup_zip_with.
-        rewrite cvLook. rewrite H1. simpl.
-        done. }
-      eassert (is_Some (physHist !! _)) as [msg physHistLook].
-      { apply elem_of_dom.
-        erewrite physAbsHistTimestamps; [ | done | done].
-        apply elem_of_dom.
-        done. }
-      iDestruct (big_sepM2_lookup with "bumperSome") as %bv; [done|done|].
-      eassert _ as temp.
-      { eapply map_Forall_lookup_1; [eapply bv|done]. }
-      destruct temp as [sNew ?].
-      iExists _, sOld, _, msg.(msg_val).
-      iDestruct (big_sepM_lookup with "offsetPts") as "$"; first done.
-      iSplitPure; first done.
-      iSplitPure; first done.
-      iSplit.
-      { iApply (big_sepM_lookup with "crashedInPts").
-        rewrite lookup_fmap.
-        erewrite slice_hist_lookup_Some; try done.
-        rewrite lookup_fmap.
-        rewrite newOffsetsLook.
-        simpl.
-        f_equiv. }
-      iFrame "pts".
-      iDestruct (big_sepM_lookup with "fragHistories") as "frags"; first done.
-      (* Note: At this point we could easily give all the fractional entries. *)
-      iDestruct (big_sepM_lookup with "frags") as "$".
-      { apply lookup_omap_Some. eexists _.
-        split; first done. rewrite drop_above_lookup_t. done. }
-      iDestruct (auth_map_map_frag_lookup_singleton with "newPhysHistFrag") as "$".
-      { rewrite /newPhysHists. rewrite lookup_fmap. rewrite /drop_all_above.
-        rewrite map_lookup_zip_with.
-        rewrite newOffsetsLook /=. rewrite physHistsLook /=.
-        done. }
-      { rewrite lookup_fmap drop_above_lookup_t physHistLook. done. }
-    }
-    iFrame "valView".
-    iSplitPure. { subst. done. }
-    (* We show the state interpretation for the high-level logic. *)
-    iExistsN.
-    rewrite /full_map.
-
-    iFrame "offsets".
-    iFrame "newPhysHists".
-    rewrite /newPhysHists /newOffsets.
-
-    rewrite slice_of_store_drop.
-
-    iFrame "ptsMap".
-    (* iFrame "offsets". *)
-    iFrame "newOrders newFullPreds newReadPreds newPersPreds hists' newAtLocs newCrashedAt".
-    iFrame "newNaLocs".
-    (* iFrame "newPhysHists". *)
-    iFrame "newBumpers".
-    iFrame "naView".
-    iFrame "fragHistories".
-    (* [oldViewsDiscarded] *)
-    iSplit.
-    { (* Showing this is easy as we have indeed discarded all views. *)
-      iIntros "!>". iApply big_sepM2_forall.
-      iSplitPure.
-      { apply dom_eq_alt_L.
-        rewrite dom_fmap_L.
-        rewrite /offsets_add /drop_all_above !dom_map_zip_with_L.
-        rewrite -offsetDom.
-        set_solver+. }
-      iPureIntro.
-      intros ??? (? & ? & ?)%lookup_fmap_Some ???? look.
-      simplify_eq.
-      apply lookup_fmap_Some in look as (? & <- & ?).
-      done. }
-
-    (* GlobalPViewPersisted *)
-    iSplit. {
-      iPoseProof (persisted_weak _ new_global_pview with "[$]") as "$".
-      apply view_le_lookup.
-      intros.
-      exists t. split; last done.
-      by apply restrict_lookup_Some in H0 as [? ?].
-    }
-
-    (* (* GlobalPView *) *)
-    (* iSplitL "globalPView"; first iFrame. *)
-    (* [locDisjoint] *)
-    iSplitPure.
-    { set_solver. }
-    (* [histDomLocs] *)
-    iSplitPure. { rewrite -domNewAbsHists. set_solver+ histDomLocs. }
-    (* [naView] *)
-    iSplitPure. { rewrite /newNaViews. apply dom_gset_to_gmap. }
-    (* mapShared. We show that the shared location still satisfy that *)
-(*     their two persist-views are equal. *)
-    iSplitPure.
-    { rewrite /shared_locs_inv.
-      rewrite /map_map_Forall.
-      eapply map_Forall_subseteq. { apply restrict_subseteq. }
-      intros ℓ hist look t newMsg histLook.
-      apply map_lookup_zip_with_Some in look as (hist' & off & -> & look & offsetsLook).
-      apply lookup_fmap_Some in look as (origHist & <- & look).
-      apply drop_all_above_lookup_Some in look as (? & ? & -> & ? & ?).
-      rewrite drop_above_fmap in histLook.
-      simplify_eq.
-      apply drop_prefix_drop_above in histLook as (-> & look).
-      apply lookup_fmap_Some in look as (? & <- & ? ).
-      split; last done.
-      destruct x1. simpl. apply view_lookup_zero_empty. }
-    (* atLocsHistories *)
-    iSplitL "atHistories".
-    { iNext.
-      iApply (big_sepM_impl with "atHistories").
-      iIntros "!>" (ℓ ? [??]%restrict_lookup_Some) "$". }
-    (* [ordered]: We show that the abstract states are still ordered. *)
-    iSplitR.
-    { iApply big_sepM2_intro.
-      { setoid_rewrite <- elem_of_dom.
-        apply set_eq.
-        rewrite restrict_dom_subset_L; first done.
-        rewrite -domHistsEqOrders.
-        set_solver+. }
-      iModIntro.
-      iModIntro.
-      iIntros (ℓ newHist order ih [ordersLook ?]%restrict_lookup_Some).
-      apply new_abs_hist_lookup_Some in ih
-          as (bumper & hist & ? & ? & ? & ? & ?).
-      simplify_eq.
-      iDestruct (big_sepM2_lookup with "ordered") as %incr; [done|done| ].
-      iDestruct (big_sepM2_lookup with "bumpMono") as %mono; [done|done| ].
-      iPureIntro.
-
-      intros ?????.
-      intros (? & ? & [??]%map_filter_lookup_Some)%lookup_omap_Some
-             (? & ? & [??]%map_filter_lookup_Some)%lookup_omap_Some.
-      eapply mono; [done | done |].
-      eapply incr; [ |done|done].
-      lia. }
-
-    (* histPViewDoms *)
-    iSplit. {
-      iPureIntro.
-      rewrite -domNewAbsHists.
-      rewrite restrict_dom_subset_L; first done.
-      set_solver.
-    }
-
-    (* for the recovery of the triple predicates, we need to process at once: *)
-(*        for each location, we need both the resource from [full] and [pers] to *)
-(*        invoke the [predsPostCrash] condition. *)
-
-    (* gathering hypotheses *)
-    iPoseProof (big_sepM2_sep_2 with "predsReadHold predsPersHold") as "predsHold".
-    iPoseProof (big_sepM2_sep_2 with "predsFullHold predsHold") as "predsHold".
-    rewrite [named "predsFullHold" _]/named [named "predsReadHold" _]/named [named "predsPersHold" _]/named.
-    rewrite bi.sep_assoc -big_sepM2_sep.
-    rewrite bi.sep_assoc -big_sepM2_sep.
-    (* now we can split the goal properly, and show that the encoded predicates *)
-(*        still holds for the new abstract history *)
-
-    iSplitL "baseMap pcRes predsHold".
-    {
-      iApply big_sepM2_later_2.
-      iDestruct (big_sepM2_impl_dom_subseteq_with_resource with "[baseMap pcRes] predsHold [#]") as "[? $]".
-      { rewrite dom_fmap_L.
-        rewrite /drop_all_above /offsets_add !dom_map_zip_with_L.
-        set_solver+. }
-      { rewrite -domNewAbsHists.
-        rewrite dom_fmap_L.
-        rewrite /drop_all_above /offsets_add !dom_map_zip_with_L.
-        rewrite /recLocs.
-        rewrite -domPhysHistsEqAbsHists.
-        rewrite -offsetDom.
-        set_solver+. }
-      { iAccu. }
-
-      iModIntro.
-      iIntros (ℓ physHist absHist newPhysHist newAbsHist physHistsLook
-               absHistsLook newPhysHistsLook newAbsHistLook).
-      iIntros "[baseMap pcRes]".
-
-      (* (* Infer what we can from the lookup in the new physical history. *) *)
-      apply lookup_fmap_Some in newPhysHistsLook as (? & ? & look).
-      apply drop_all_above_lookup_Some in look as (newOffset & ? & -> & newOffsetLook & ?).
-      simplify_eq.
-      eassert _ as eq by apply newOffsetLook.
-      apply map_lookup_zip_with_Some in eq as (oldOffset & [tC] &?&?& cvLook).
-
-      (* Infer what we can from the lookup in the new abstract history. *)
-      apply new_abs_hist_lookup_Some in newAbsHistLook
-        as (bumper & ? & ? & offsetLook & ? & ? & bumpersLook).
-      rewrite /newOffsets in offsetLook.
-      simplify_eq.
-
-      iIntros "((%predFull & % & %predsFullLook & % & fullEncs) &
-                (%predRead & % & %predsReadLook & % & readEncs) &
-                (%predPers & %old_ts & %old_pers_encS & %old_pers_msg &
-                 %predsPersLook & %globalPViewLook & %absHistPersLook &
-                 %physHistPersLook & persEnc))".
-      simplify_eq.
-
-      distrib_later.
-      pull_left (▷ (∃ _ _, ⌜newFullPreds !! _ = _⌝ ∗ _))%I.
-
-      set (tCrash := oldOffset + tC).
-      (* predsFull *)
-      rewrite bi.later_exist bi.sep_exist_r.
-      iExists predFull.
-      rewrite bi.later_exist bi.sep_exist_r.
-
-      iExists (tCrash).
-      iAssert (⌜newFullPreds !! ℓ = Some predFull⌝)%I as "$". {
-        iPureIntro.
-        rewrite /newFullPreds.
-        apply restrict_lookup_Some_2; first done.
-        apply elem_of_dom_2 in cvLook.
-        apply elem_of_dom_2 in absHistsLook.
-        set_solver+ cvLook absHistsLook. }
-      rewrite bi.later_sep -bi.sep_assoc.
-      iSplitPure; first done.
-      (* predsRead *)
-      pull_left (▷ (∃ _ _, ⌜newReadPreds !! _ = _⌝ ∗ _))%I.
-      rewrite bi.later_exist bi.sep_exist_r.
-      iExists predRead.
-      rewrite bi.later_exist bi.sep_exist_r.
-      iExists (tCrash).
-      iAssert (⌜newReadPreds !! ℓ = Some predRead⌝)%I as "$". {
-        iPureIntro.
-        rewrite /newReadPreds.
-        apply restrict_lookup_Some_2; first done.
-        apply elem_of_dom_2 in cvLook.
-        apply elem_of_dom_2 in absHistsLook.
-        set_solver+ cvLook absHistsLook. }
-      rewrite bi.later_sep -bi.sep_assoc.
-      iSplitPure; first done.
-
-      (* predsPers *)
-      pull_left (▷ (∃ _ _ _ _, _))%I.
-      rewrite bi.later_exist bi.sep_exist_r.
-      iExists predPers.
-      rewrite bi.later_exist bi.sep_exist_r.
-      iExists (tCrash).
-      rewrite bi.later_exist bi.sep_exist_r.
-      (* obtains the encoded state through valid_slice *)
-      iAssert (∃ encS, ⌜ omap bumper (drop_above (tCrash) absHist)!!
-                      (tCrash)%nat = Some encS ⌝)%I
-        as (new_encS) "%". {
-        apply (slice_hist_Some _ _ ℓ (tCrash) absHist)
-          in cvSlicesAbsHists as (encS & absHistLook & ?);
-          [ | | done ].
-        2: {
-          rewrite lookup_fmap_Some.
-          eexists.
-          split; done.
-        }
-        iPoseProof (big_sepM2_lookup_acc with "bumperSome")
-          as "[%bumperLook _]";
-          [exact absHistsLook | exact bumpersLook | ].
-        iPureIntro.
-        pose proof (map_Forall_lookup_1 _ _ _ _ bumperLook absHistLook)
-          as [encS' ?].
-        rewrite map_Forall_lookup /is_Some in bumperLook.
-        eexists.
-        rewrite lookup_omap_Some.
-        eexists.
-        rewrite drop_above_lookup_t.
-        done.
-      }
-      iExists new_encS.
-      (* for some reason, [bi.later_exist] fail with typeclasses... *)
-      rewrite -bi.later_exist_2 bi.sep_exist_r.
-      assert (∃ msg, (drop_above (tCrash) physHist) !! (tCrash)%nat = Some msg)
-        as [new_msg newMsgLook]. {
-        pose proof (slice_hist_Some _ _ ℓ tC (drop_prefix physHist oldOffset)
-                      cvSlicesPhysHists
-                      ltac:(done)
-                      ltac:(rewrite map_lookup_zip_with_Some;
-                            eexists _, _; done)) as [msg [physHistLook _]].
-        rewrite drop_prefix_lookup in physHistLook. rewrite Nat.add_comm in physHistLook.
-        eexists.
-        rewrite drop_above_lookup_t.
-        done.
-      }
-      iExists (discard_msg_views new_msg).
-      iAssert (⌜newPersPreds !! ℓ = Some predPers⌝)%I as "$".
-      { iPureIntro.
-        rewrite /newPersPreds.
-        apply restrict_lookup_Some_2; first done.
-        apply elem_of_dom_2 in cvLook.
-        apply elem_of_dom_2 in absHistsLook.
-        set_solver+ cvLook absHistsLook. }
-
-      (* [iFrame "%"] takes too long on my computer, *)
-(*          therefore I'm refactoring the goal here *)
-      do ? lazymatch goal with
-             | |- context [ ((_ ∗ _) ∗ _)%I ] => rewrite -bi.sep_assoc
-             | |- context [ (▷ (_ ∗ _))%I ] => rewrite bi.later_sep
-             end.
-
-      iSplitPure. {
-        left.
-        rewrite /offsets_add.
-        rewrite map_lookup_zip_with_Some.
-        eexists. exists (MaxNat 0).
-        split; first done.
-        split.
-        - rewrite map_lookup_zip_with_Some.
-          exists oldOffset, (MaxNat tC).
-          done.
-        - rewrite restrict_lookup_Some.
-          rewrite (view_to_zero_lookup _ _ (MaxNat tC)); last done.
-          split; first done.
-          rewrite elem_of_intersection.
-          split; eapply elem_of_dom_2; done.
-      }
-      iSplitPure; first done.
-      iSplitPure; first by (rewrite lookup_fmap_Some; eexists).
-
-      iDestruct (big_sepM2_dom with "fullEncs") as %physEncDomEq.
-      iDestruct (big_sepM2_lookup with "bumperSome") as %map; [done|done|].
-
-      rewrite -2!big_sepM2_later_2.
-      pull_left ([∗ map] _↦ _; _ ∈ _; _, ▷ (_ -∗ ⌜ _ = None ⌝ -∗ _))%I.
-      iApply bi.wand_frame_r. {
-        iApply (big_sepM_singleton_hold _ _ _ (tCrash));
-          [ | | by rewrite lookup_fmap_Some; eexists | done ].
-        2: {
-          rewrite dom_fmap_L.
-          rewrite dom_omap_id_L; first by apply drop_above_dom_eq.
-          eapply (map_Forall_subseteq); first apply map_filter_subseteq.
-          apply map; done.
-        }
-        rewrite dom_fmap_L.
-        iIntros (???? elemOf) "_". iModIntro. iIntros.
-        rewrite elem_of_dom in elemOf.
-        rewrite drop_above_lookup_gt in elemOf; last by lia.
-        apply is_Some_None in elemOf.
-        done.
-      }
-      iSimpl.
-
-      rewrite -2!bi_wand_drop_premise.
-
-      assert (default ∅ (newNaViews !! ℓ) = ∅) as ->. {
-        rewrite /newNaViews.
-        destruct (gset_to_gmap ∅ newNaLocs !! ℓ) eqn:eq.
-        - apply lookup_gset_to_gmap_Some in eq as [_ ->]. done.
-        - done.
-      }
-
-      (* calculate the state for maximal timestamp (the full timestamp we will use) *)
-      set t_full := max_msg physHist.
-      assert (is_Some $ physHist !! t_full) as [full_msg physHistFullLook]. {
-        apply elem_of_dom.
-        rewrite /max_msg.
-        apply elem_of_elements.
-        apply max_list_elem_of.
-        apply elem_of_dom_2 in physHistPersLook.
-        apply elem_of_elements in physHistPersLook.
-        eapply elem_of_not_nil.
-        done.
-      }
-
-      assert (is_Some $ absHist !! t_full) as [full_encS absHistFullLook]. {
-        apply elem_of_dom.
-        rewrite /max_msg.
-        apply elem_of_elements.
-        rewrite -physEncDomEq.
-        apply max_list_elem_of.
-        apply elem_of_dom_2 in physHistPersLook.
-        apply elem_of_elements in physHistPersLook.
-        eapply elem_of_not_nil.
-        done.
-      }
-
-      (* lookup for read states (at crash timestamp) *)
-      assert (is_Some $ physHist !! (tCrash)) as [read_msg physHistReadLook]. {
-        rewrite /tCrash -Nat.add_comm.
-        rewrite -drop_prefix_lookup.
-        eapply valid_slice_lookup; [ exact cvSlicesPhysHists | done | ].
-        apply map_lookup_zip_with_Some.
-        by exists physHist, oldOffset.
-      }
-
-      assert (is_Some $ absHist !! (tCrash)) as [crash_encS absHistCrashLook]. {
-        rewrite /tCrash -Nat.add_comm.
-        rewrite -drop_prefix_lookup.
-        rewrite -valid_slice_drop_prefix in cvSlicesAbsHists.
-        eapply valid_slice_lookup; [ exact cvSlicesAbsHists | done | ].
-        apply map_lookup_zip_with_Some.
-        by exists absHist, oldOffset.
-      }
-
-      (* We try to allocate all the predicates for the next generation *)
-(*        * first, all [read] predicates except for the [tCrash] predicate are still *)
-(*        * allocated [read]. *)
-(*        * second, the pers predicate, the read predicate at [tCrash], and one of the *)
-(*        * full predicate after [tCrash] are allocated for the full recovery *)
-(*        * third, all full predicates before [tCrash] are reduced to [read] predicates *)
-(*        * for the next generation. *)
-(*        * *)
-
-      (* The crash timestamp is special for read predicates *)
-      iPoseProof (big_sepM2_delete with "readEncs") as "[readEncAtCrash readEncs]";
-        [ eassumption | done | ].
-      iPoseProof ((big_sepM2_split (λ t _ _, tCrash ≤ t)) with "fullEncs")
-        as "[fullAfterCrash fullBeforeCrash]".
-
-      rewrite [(▷ _ ∗ ▷ _ ∗ _)%I]bi.sep_assoc.
-      iApply (wand_passthrough with "[] [] [baseMap pcRes] [persEnc fullAfterCrash readEncAtCrash] [readEncs fullBeforeCrash]");
-        [ | | iAccu | iAccu | iAccu ].
-      { (* proof for full and pers *)
-        iIntros "((persEnc & fullEncs & readEncAtCrash) & baseMap & pcRes)".
-        iPoseProof ((big_sepM2_delete _ _ _ tCrash) with "fullEncs") as "[fullEncAtCrash fullEncs]";
-          [ done | done | ].
-        iSpecialize ("fullEncAtCrash" with "[//]").
-        iDestruct (big_sepM2_lookup with "predFullPostCrash")
-          as (pred_read' pred_pers' order) "(% & % & %orderLook & postCrash)";
-          [ apply predsFullLook | apply bumpersLook | ].
-        rewrite drop_above_lookup_t in newMsgLook.
-        rewrite lookup_omap drop_above_lookup_t absHistCrashLook in H0.
-        simplify_eq.
-        (* case distinction on whether we crashed at the full timestamp *)
-        destruct (Nat.eq_dec t_full (tCrash)) as [ Heq | ? ].
-        - (* we crash at [t_full] *)
-          iClear "readEncAtCrash fullEncs".
-          (* lookup for full predicate *)
-          simplify_eq.
-          iSpecialize ("fullEncAtCrash" with "[%] [%]");
-            [ lia | by rewrite -Nat.add_1_r -Heq lookup_max_msg_succ | ].
-          rewrite -> Heq in *.
-          simplify_eq.
-          (* we will use the join view for [predPostCrash] *)
-          set V_pers := (v in encoded_predicate_holds _ old_pers_encS _ (v, _)).
-          set V_full := (v in encoded_predicate_holds _ full_encS _ (v, _)).
-          pose proof (thread_view_le_l V_pers V_full).
-          assert ((V_pers, hGD) ⊑ (V_pers ⊔ V_full, hGD)) by (split; [ apply thread_view_le_l | done ]).
-          rewrite [encoded_predicate_holds _ _ _ (V_pers, _)]encoded_predicate_holds_mono; last done.
-          assert ((V_full, hGD) ⊑ (V_pers ⊔ V_full, hGD)) by (split; [ apply thread_view_le_r | done ]).
-          rewrite [encoded_predicate_holds _ _ _ (V_full, _)]encoded_predicate_holds_mono; last done.
-          iSpecialize ("postCrash" $! old_pers_encS old_pers_msg.(msg_val)
-                        with "[$persEnc]").
-          iDestruct "postCrash" as "[postCrash _]".
-          iSpecialize ("postCrash" $! full_encS _ full_msg.(msg_val) with "fullEncAtCrash").
-          iDestruct ("postCrash" with "[//]") as (P_full P_pers) "(#fullEq & #persEq & pred)".
-          iSimpl in "pred".
-          iDestruct ("pred" $! _ _ bumpers na_views store _
-                      with "persImpl baseMap") as "(baseMap & pred)".
-          iDestruct ("pred" with "[$pcResPers $pcRes]") as "[H pcRes]".
-          iFrame.
-          setoid_rewrite <- bi.later_exist_2.
-          rewrite bi.sep_exist_r.
-          iExists _.
-          distrib_later.
-          pull_left (▷ (_ ≡ Some _))%I.
-          iSplit; first done.
-          pull_left (∃ _, _)%I.
-          rewrite bi.sep_exist_r.
-          iExists _.
-          distrib_later.
-          pull_left (▷ (_ ≡ Some _))%I.
-          iSplit; first done.
-          iFrame.
-          rewrite -bi.later_sep.
-          rewrite [(P_pers _ ∗ _)%I] bi.sep_comm.
-          iNext.
-          iSpecialize ("H" $! CV).
-          rewrite monPred_wand_force.
-          monPred_simpl.
-          iApply "H".
-          iSimpl.
-          iFrame "newCrashedAt".
-          assert (msg_persisted_after_view full_msg ⊑ CV). {
-            eapply consistent_cut_extract; [done | done | | |  ].
-            - eapply lookup_weaken; last done.
-              apply map_lookup_zip_with_Some.
-              eexists _, _. split_and!; done.
-            - apply drop_prefix_lookup_Some_2.
-              rewrite Nat.add_comm.
-              done.
-            - lia.
-          }
-          assert (msg_persisted_after_view old_pers_msg ⊑ CV). {
-            destruct globalPViewLook as [globalPViewLook | [? ?]].
-            - rewrite map_lookup_zip_with_Some in globalPViewLook.
-              destruct globalPViewLook as (? & [?] & ? & ? & globalPViewLook).
-              simplify_eq.
-              eapply consistent_cut_extract; [done | done | | |  ].
-              + eapply lookup_weaken; last done.
-                apply map_lookup_zip_with_Some.
-                eexists _, _. split_and!; done.
-              + apply drop_prefix_lookup_Some_2.
-                rewrite Nat.add_comm.
-                done.
-              + assert (global_pview ≼ CV) as view_included by (by etrans).
-                rewrite lookup_included in view_included.
-                rewrite -Some_MaxNat_included -cvLook -globalPViewLook.
-                done.
-            - eapply consistent_cut_extract; [done | done | | |  ].
-              + eapply lookup_weaken; last done.
-                apply map_lookup_zip_with_Some.
-                eexists _, _. split_and!; done.
-              + apply drop_prefix_lookup_Some_2.
-                rewrite Nat.add_comm.
-                rewrite [old_ts]plus_n_O in physHistPersLook.
-                done.
-              + lia.
-          }
-          iSplitPure; first by apply view_lub_le.
-          iApply (persisted_weak with "pers").
-          f_equiv.
-          by apply view_lub_le.
-        - (* we crash at some other timestamps, we should use the second rule *)
-          (* but first, we need to sort out the proper thread view *)
-          iPoseProof (big_sepM2_lookup with "fullEncs [%] [%] [%]") as "fullEnc";
-            do ? (rewrite lookup_delete_ne; last done);
-            [ apply physHistFullLook |
-              apply absHistFullLook | | |
-              by rewrite -Nat.add_1_r lookup_max_msg_succ | ].
-            { apply max_list_elem_of_le.
-              rewrite elem_of_elements elem_of_dom.
-              by eexists. }
-            { apply (Nat.le_trans _ old_ts).
-              - destruct globalPViewLook as [globalPViewLook | []].
-                + rewrite map_lookup_zip_with_Some in globalPViewLook.
-                  destruct globalPViewLook as (x & [] & ? & ? & ?).
-                  simplify_eq.
-                  lia.
-                + simplify_eq.
-                  lia.
-              - apply max_list_elem_of_le.
-                apply elem_of_elements.
-                apply elem_of_dom.
-                by exists old_pers_msg. }
-          set V_pers := (v in encoded_predicate_holds _ old_pers_encS _ (v, _)).
-          set V_read := (v in encoded_predicate_holds _ crash_encS _ (v, _)).
-          iAssert (encoded_predicate_holds predRead crash_encS (msg_val read_msg) (V_read, hGD))%I
-            with "[readEncAtCrash fullEncAtCrash]" as "readEnc". {
-            assert (oldOffset ≤ tCrash) by lia.
-            destruct (physHist !! S tCrash).
-            - iApply "readEncAtCrash".
-              iPureIntro; right; done.
-            - iDestruct (big_sepM2_lookup with "predFullReadSplit") as "#split"; [ done | done | ].
-              iSpecialize ("fullEncAtCrash" with "[%] [//]"); first lia.
-              iApply "split".
-              iFrame.
-          }
-          assert ((V_pers, hGD) ⊑ (V_pers ⊔ V_read, hGD)) by (split; [ apply thread_view_le_l | done ]).
-          rewrite [encoded_predicate_holds _ _ _ (V_pers, _)]encoded_predicate_holds_mono; last done.
-          assert ((V_read, hGD) ⊑ (V_pers ⊔ V_read, hGD)) by (split; [ apply thread_view_le_r | done ]).
-          rewrite [encoded_predicate_holds _ _ _ (V_read, _)]encoded_predicate_holds_mono; last done.
-          iSpecialize ("postCrash" $! old_pers_encS old_pers_msg.(msg_val) with "[$persEnc]").
-          iDestruct "postCrash" as "[_ postCrash]".
-          iDestruct (big_sepM2_lookup with "ordered") as "%ordered"; [ done | done | ].
-          iDestruct "fullEnc" as (P_full) "[#eqPFull PFullHolds]".
-          iDestruct ("postCrash" $! full_encS crash_encS new_encS full_msg.(msg_val) read_msg.(msg_val) P_full
-                        with "[$]") as (P_obj) "[PFullImplObj postCrash]".
-          rewrite monPred_at_objectively.
-          iSpecialize ("PFullImplObj" with "PFullHolds").
-          rewrite monPred_at_objectively.
-          iSpecialize ("PFullImplObj" $! (V_pers ⊔ V_read, hGD)).
-          iDestruct ("postCrash" with "[$PFullImplObj] [//] [%] [%] [$readEnc]")
-            as (P_full' P_pers') "(#eqFull & #eqPers & pred)".
-          { assert (old_ts ≤ tCrash). {
-              rewrite map_lookup_zip_with_Some in globalPViewLook.
-              destruct globalPViewLook as [globalPViewLook | []].
-              - destruct globalPViewLook as (? & [?] & ? & ? & globalPViewLook).
-                simplify_eq.
-                apply plus_le_compat_l.
-                rewrite -Some_MaxNat_included -cvLook -globalPViewLook.
-                assert (global_pview ≼ CV) as view_included by (by etrans).
-                rewrite lookup_included in view_included.
-                done.
-              - simplify_eq.
-                lia.
-            }
-            destruct (Nat.eq_dec old_ts tCrash); [simplify_eq; by right | left].
-            eapply ordered; [ | done | done ].
-            lia. }
-          { assert (tCrash ≤ t_full). {
-              apply max_list_elem_of_le.
-              rewrite elem_of_elements elem_of_dom.
-              by eexists.
-            }
-            eapply ordered; [ | done | done ].
-            lia. }
-          iEval (simpl) in "pred".
-          iDestruct ("pred" $! _ _ bumpers na_views store _
-                      with "persImpl baseMap") as "(baseMap & pred)".
-          iDestruct ("pred" with "[$pcResPers $pcRes]") as "[H pcRes]".
-          iFrame.
-          setoid_rewrite <- bi.later_exist_2.
-          rewrite bi.sep_exist_r.
-          iExists _.
-          distrib_later.
-          pull_left (▷ (_ ≡ Some _))%I.
-          iSplit; first done.
-          pull_left (∃ _, _)%I.
-          rewrite bi.sep_exist_r.
-          iExists _.
-          distrib_later.
-          pull_left (▷ (_ ≡ Some _))%I.
-          iSplit; first done.
-          iFrame.
-          rewrite -bi.later_sep.
-          rewrite [(P_pers' _ ∗ _)%I] bi.sep_comm.
-          iNext.
-          iSpecialize ("H" $! CV).
-          rewrite monPred_wand_force.
-          monPred_simpl.
-          iApply "H".
-          iSimpl.
-          iFrame "newCrashedAt".
-          assert (msg_persisted_after_view read_msg ⊑ CV). {
-            eapply consistent_cut_extract; [done | done | | |  ].
-            - eapply lookup_weaken; last done.
-              apply map_lookup_zip_with_Some.
-              eexists _, _. split_and!; done.
-            - apply drop_prefix_lookup_Some_2.
-              rewrite Nat.add_comm.
-              done.
-            - lia.
-          }
-          assert (msg_persisted_after_view old_pers_msg ⊑ CV). {
-            rewrite map_lookup_zip_with_Some in globalPViewLook.
-            destruct globalPViewLook as [globalPViewLook | []].
-            - destruct globalPViewLook as (? & [] & ? & ? & GlobalPViewLook).
-              simplify_eq.
-              eapply consistent_cut_extract; [done | done | | |  ].
-              + eapply lookup_weaken; last done.
-                apply map_lookup_zip_with_Some.
-                eexists _, _. split_and!; done.
-              + apply drop_prefix_lookup_Some_2.
-                rewrite Nat.add_comm.
-                done.
-              + assert (global_pview ≼ CV) as view_included by (by etrans).
-                rewrite lookup_included in view_included.
-                rewrite -Some_MaxNat_included -cvLook -GlobalPViewLook.
-                done.
-            - eapply consistent_cut_extract; [done | done | | |  ].
-              + eapply lookup_weaken; last done.
-                apply map_lookup_zip_with_Some.
-                eexists _, _. split_and!; done.
-              + apply drop_prefix_lookup_Some_2.
-                rewrite Nat.add_comm.
-                rewrite [old_ts]plus_n_O in physHistPersLook.
-                done.
-              + lia.
-          }
-          iSplitPure; first by apply view_lub_le.
-          iApply (persisted_weak with "pers").
-          f_equiv.
-          by apply view_lub_le.
-      }
-      {
-        iIntros "([readEncs fullEncs] & baseMap & pcRes)".
-        rewrite [([∗ map] _ ↦ _; _ ∈ _; _, ▷ _)%I](big_sepM2_delete _ _ _ tCrash);
-        [ | rewrite lookup_fmap_Some; by eexists | done ].
-        rewrite [(discard_msg_views <$> _) !! _]lookup_fmap drop_above_lookup_gt; last lia.
-        pull_left (▷ _)%I.
-        iSplitL "". {
-          iIntros "!>" (Hcontra).
-          destruct Hcontra as [ | Hcontra ]; [ lia | by apply is_Some_None in Hcontra ].
-        }
-        pull_right ([∗ map] _ ↦ _; _ ∈ _; _, _)%I.
-
-        (* merge full predicates and read predicates into one single [∗ map] for *)
-(*          * the next lemma. *)
-        iPoseProof (big_sepM2_delete _ _ _ tCrash with "fullEncs") as "[_ fullEncs]";
-          [ done | done | ].
-        iPoseProof (big_sepM2_sep_2 with "readEncs fullEncs") as "encs".
-
-        iApply (big_sepM2_impl_dom_subseteq_with_resource with "[baseMap pcRes] encs").
-        {
-          rewrite 2!dom_delete.
-          rewrite dom_fmap_L.
-          apply difference_mono_r.
-          apply dom_filter_subseteq.
-        }
-        {
-          rewrite 2!dom_delete_L.
-          rewrite dom_fmap_L.
-          erewrite drop_above_dom_eq; last apply physEncDomEq.
-          rewrite dom_omap_id_L; first done.
-          eapply map_Forall_subseteq; last apply map.
-          apply map_filter_subseteq.
-        }
-        { iFrame. }
-        iIntros "!>" (t msg oldS ? newS physHistLook absHistLook).
-        assert (tCrash ≠ t) by (by apply lookup_delete_Some in physHistLook as [? _]).
-        rewrite ?(lookup_delete_ne _ tCrash t ltac:(done)).
-        rewrite lookup_delete_ne in physHistLook; last done.
-        rewrite lookup_delete_ne in absHistLook; last done.
-        iIntros ((? & <- & look)%lookup_fmap_Some bumperLook).
-        apply map_filter_lookup_Some in look as [??].
-        apply lookup_omap_Some in bumperLook as (? & ? & (? & ?)%map_filter_lookup_Some).
-        simplify_eq.
-        iIntros "[baseMap pcRes] [predReadHolds predFullHolds]".
-        iSpecialize ("predFullHolds" with "[%]"); first lia.
-        pull_left (▷ _)%I.
-        iAssert (encoded_predicate_holds predRead oldS (msg_val msg)
-                   (default (msg_store_view msg) (na_views !! ℓ),
-                      msg_persisted_after_view msg, ∅, hGD))%I
-          with "[predReadHolds predFullHolds]" as "predReadHolds". {
-          destruct (decide (oldOffset ≤ t ∧ physHist !! S t = None)) as [ [] | yes ].
-          - iSpecialize ("predFullHolds" with "[//] [//]").
-            iPoseProof (big_sepM2_lookup with "predFullReadSplit predFullHolds") as "split";
-              [ done | done | ].
-            iFrame.
-          - iApply ("predReadHolds" with "[%]").
-            apply not_and_l in yes as [ | ].
-            + left. lia.
-            + right. by destruct (physHist !! S t) eqn:Heqn.
-        }
-        (* It's time to lookup the postcrash invariant *)
-        iDestruct (big_sepM2_lookup with "predReadPostCrash [//] [$predReadHolds]")
-          as (?P) "[#predEq pred]"; [apply predsReadLook | apply bumpersLook | ].
-        iEval (simpl) in "pred".
-        iDestruct ("pred" $! _ _ bumpers na_views store _
-                    with "persImpl baseMap") as "(baseMap & pred)".
-        iDestruct ("pred" with "[$pcResPers $pcRes]") as "[H pcRes]".
-        iFrame.
-        iIntros "!>" (_).
-        iExists _.
-        iFrame "#".
-        iEval (simpl).
-        assert (default ∅ (newNaViews !! ℓ) = ∅) as ->. {
-          rewrite /newNaViews.
-          destruct (gset_to_gmap ∅ newNaLocs !! ℓ) eqn:eq.
-          - apply lookup_gset_to_gmap_Some in eq as [_ ->]. done.
-          - done.
-        }
-        iApply ("H" $! CV).
-        iSimpl.
-        iFrame "newCrashedAt".
-        iDestruct (big_sepM2_lookup with "oldViewsDiscarded") as %disc; [done | done | ].
-        assert (msg_persisted_after_view msg ⊑ CV). {
-          assert (t < oldOffset ∨ oldOffset ≤ t) as [? | le] by lia.
-          { eassert _ as eq by (by eapply disc).
-            rewrite -eq.
-            apply view_empty_least. }
-          apply Nat.le_exists_sub in le as (tt & eq & ?).
-          eapply consistent_cut_extract; [done | done | | |  ].
-          - eapply lookup_weaken; last done.
-            apply map_lookup_zip_with_Some.
-            eexists _, _. split_and!; done.
-          - apply drop_prefix_lookup_Some_2.
-            erewrite <- eq.
-            done.
-          - lia.
-        }
-        iSplitPure; first done.
-        iApply (persisted_weak with "pers").
-        f_equiv.
-        done.
-      }
-    }
-    (* [bumpMono] - Show that the bumpers are still monotone. *)
-    iSplitR "".
-    { iApply (big_sepM2_impl_subseteq with "bumpMono").
-      { apply restrict_subseteq. }
-      { apply restrict_subseteq. }
-      { rewrite /newOrders /newBumpers.
-        rewrite 2!restrict_dom_L.
-        rewrite -domOrdersEqBumpers.
-        done. } }
-    (* domain equations *)
-    do 3 (iSplitPure; first (rewrite 2!restrict_dom_L; congruence)).
-
-    (* [predPostCrash] - a little bit more complicated due to we look up more than two maps now *)
-    iSplitR "". {
-      iApply big_sepM2_impl. {
-        iApply (big_sepM2_impl_subseteq with "predFullPostCrash").
-        { by apply restrict_subseteq. }
-        { by apply restrict_subseteq. }
-        { rewrite 2!restrict_dom_L.
-          rewrite -FullBumperDoms.
-          done. }
-      }
-      { iIntros "!> !>" (ℓ predFull bumper) "%predFullLook %bumperLook
-        (%predRead & %predPers & %order & %predReadLook & %predPersLook & %orderLook & ?)".
-        iExists predRead, predPers, order.
-        assert (ℓ ∈ recLocs). {
-          rewrite restrict_lookup_Some in predFullLook.
-          tauto.
-        }
-        do 3 (iSplitPure; first by rewrite restrict_lookup_elem_of).
-        iFrame.
-      }
-    }
-
-    (* [predReadPostCrash] *)
-    iSplitR "". {
-      iApply (big_sepM2_impl_subseteq with "predReadPostCrash").
-      { by apply restrict_subseteq. }
-      { by apply restrict_subseteq. }
-      { rewrite 2!restrict_dom_L.
-        rewrite -ReadBumperDoms.
-        done. }
-    }
-    (* [predFullReadSplit] *)
-    iSplitR "". {
-      iApply (big_sepM2_impl_subseteq with "predFullReadSplit").
-      { by apply restrict_subseteq. }
-      { by apply restrict_subseteq. }
-      { rewrite 2!restrict_dom_L.
-        rewrite ReadBumperDoms FullBumperDoms.
-        done. }
-    }
-    (* bumperBumpToValid *)
-    iSplitPure.
-    { eapply map_Forall_subseteq; last done.
-      apply restrict_subseteq. }
-    (* bumperSome *)
-    { iApply big_sepM2_forall.
-      iSplitPure.
-      { apply dom_eq_alt_L.
-        rewrite restrict_dom_subset_L; first done.
-        rewrite /recLocs.
-        rewrite domHistsEqBumpers.
-        set_solver+. }
-      iIntros (ℓ hist bumper look look2).
-      apply new_abs_hist_lookup_Some in look.
-      destruct look as (bumper' & s & ? & hist' & ? & ? & ?).
-      simplify_eq.
-      assert (bumper = bumper') as <-.
-      { eapply lookup_weaken_inv; [done| |done]. apply restrict_subseteq. }
-      iNext. iIntros (?? look).
-      iDestruct (big_sepM2_lookup with "bumperSome") as %i; [done|done|].
-      apply lookup_omap_Some in look as (? & ? & (? & ?)%map_filter_lookup_Some).
-      eapply map_Forall_lookup_1 in i as [bumpedS eq]; last done.
-      simplify_eq.
-      eapply map_Forall_lookup_1 in bumperBumpToValid as [spa equi]; last done; first done.
-      rewrite equi.
-      done. }
-  Qed.
+(*     iIntros ([store PV CV pIncl cut]) "[nvm_heap extra]". *)
+(*     iMod (heap_ctx_next_generation with "nvm_heap") as "nvm_heap"; first done. *)
+(*     do 3 iModIntro. *)
+
+
+(*     iIntros ([store PV CV pIncl cut]). *)
+(*     iIntros "[H1 H2] P". *)
+(*     iNamed "H1". iNamed "H2". *)
+
+(*     (* Our [phys_hist] may contain only a subset of all the locations in *) *)
+(* (*     [store]. But, those that are in [phys_hist] agree with what is in *) *)
+(* (*     [store]. *) *)
+(*     iAssert (⌜ map_zip_with drop_prefix phys_hists offsets ⊆ store  ⌝)%I *)
+(*       as %physHistsSubStore. *)
+(*     { rewrite map_subseteq_spec. *)
+(*       iIntros (ℓ hist look). *)
+(*       iDestruct (big_sepM_lookup with "ptsMap") as "pts"; first eassumption. *)
+(*       iApply (gen_heap_valid with "Hσ pts"). } *)
+
+(*     (* TODO: find a better place *) *)
+(*     iAssert (⌜ global_pview ⊑ PV ⌝)%I as "%pviewPV"; *)
+(*       first by iApply (persisted_auth_included with "Hpers"). *)
+
+(*     (* We need to first re-create the ghost state for the base *) *)
+(* (*     interpretation. *) *)
+(*     iMod (nvm_heap_reinit _ _ _ _ _ γcrash with "Hσ Hpers") *)
+(*       as (hGD') "(%crEq & valView & baseMap & baseInterp & #persImpl & #pers & *)
+(*                             #newCrashedAt)"; *)
+(*       try done. *)
+
+(*     iDestruct (or_lost_post_crash_full with "newCrashedAt pers") as "#orLost". *)
+
+(*     iDestruct (big_sepM2_dom with "ordered") as %domHistsEqOrders. *)
+(*     iDestruct (big_sepM2_dom with "bumpMono") as %domOrdersEqBumpers. *)
+(*     iDestruct (big_sepM2_dom with "bumperSome") as %domHistsEqBumpers. *)
+(*     iDestruct (big_sepM2_dom with "predsFullHold") as %domPhysHistsEqAbsHists. *)
+(*     iDestruct (big_sepM2_dom with "oldViewsDiscarded") as %offsetDom. *)
+
+(*     (* A name for the set of recovered locations. Per the above equalities this *) *)
+(* (*     set could be expressed in a number of other ways (for instance by using *) *)
+(* (*     [phys_hists] instead of [abs_hists].)*) *)
+(*     set (recLocs := dom CV ∩ dom abs_hists). *)
+
+(*     set newOffsets := offsets_add offsets CV. *)
+
+(*     (* The new offsets is a valid slice of the abstract history. This should *) *)
+(* (*     follow from the relationship between [phys_hists] and the points-to *) *)
+(* (*     predicates and the fact that [CV] is a valid slice of these. *) *)
+
+(*     set (newAbsHists := new_abs_hist abs_hists newOffsets bumpers). *)
+
+(*     iMod (full_map_alloc newAbsHists) *)
+(*       as (new_abs_history_name) "(hists' & knowHistories & #fragHistories)". *)
+
+(*     assert (recLocs = (dom newOffsets)) as domNewOffsets. *)
+(*     { rewrite dom_map_zip_with_L. *)
+(*       rewrite -offsetDom. rewrite domPhysHistsEqAbsHists. set_solver+. } *)
+(*     assert (recLocs = (dom newAbsHists)) as domNewAbsHists. *)
+(*     { rewrite new_abs_hist_dom. *)
+(*       rewrite -domHistsEqBumpers. *)
+(*       rewrite domNewOffsets. *)
+(*       set_solver. } *)
+(*     (* Allocate new ghost state for the logical histories. *) *)
+(*     rewrite /interp. *)
+
+(*     (* We freeze/persist the old authorative resource algebra. *) *)
+(*     iMod (ghost_map_auth_persist with "allOrders") as "#allOrders". *)
+(*     iMod (ghost_map_auth_persist with "offsets") as "#oldOffsets". *)
+(*     (* iMod (own_update with "globalPView") as "oldGlobalPView". *) *)
+(*     (* { apply auth_update_auth_persist. } *) *)
+(*     (* iDestruct "oldGlobalPView" as "#oldGlobalPView". *) *)
+(*     iMod (own_update with "atLocs") as "atLocs". *)
+(*     { apply auth_update_auth_persist. } *)
+(*     iDestruct "atLocs" as "#atLocs". *)
+(*     iMod (own_update with "naLocs") as "naLocs". *)
+(*     { apply auth_update_auth_persist. } *)
+(*     iDestruct "naLocs" as "#naLocs". *)
+(*     iMod (own_all_bumpers_persist with "allBumpers") as "#oldBumpers". *)
+(*     iMod (own_update with "full_predicates") as "allFullPredicates". *)
+(*     { apply auth_update_auth_persist. } *)
+(*     iDestruct "allFullPredicates" as "#allFullPredicates". *)
+(*     iMod (own_update with "read_predicates") as "allReadPredicates". *)
+(*     { apply auth_update_auth_persist. } *)
+(*     iDestruct "allReadPredicates" as "#allReadPredicates". *)
+(*     iMod (own_update with "pers_predicates") as "allPersPredicates". *)
+(*     { apply auth_update_auth_persist. } *)
+(*     iDestruct "allPersPredicates" as "#allPersPredicates". *)
+(*     (* iDestruct "history" as "[fullHist1 fullHist2]". *) *)
+(*     iMod (full_map_persist with "history") as "#oldFullHist". *)
+(*     (* iMod (own_update with "fullHist2") as "oldFullHist2". *) *)
+(*     (* { apply auth_update_auth_persist. } *) *)
+(*     (* iDestruct "oldFullHist2" as "#oldFullHist2". *) *)
+(*     (* Ghost state for physical history. *) *)
+(*     iMod (own_update with "physHist") as "oldPhysHist". *)
+(*     { apply auth_update_auth_persist. } *)
+(*     iDestruct "oldPhysHist" as "#oldPhysHist". *)
+(*     iMod (ghost_map_auth_persist with "naView") as "#oldNaView". *)
+
+(*     (* Some locations may be lost after a crash. For these we need to *) *)
+(* (*     forget/throw away the predicate and preorder that was choosen for the *) *)
+(* (*     location. *) *)
+(*     set newOrders := restrict recLocs orders. *)
+(*     iMod (own_all_preorders_gname_alloc newOrders) *)
+(*       as (new_orders_name) "[newOrders #fragOrders]". *)
+
+(*     iMod (ghost_map_alloc_persistent newOffsets) as *)
+(*       (new_offset_name) "[offsets #offsetPts]". *)
+
+(*     set new_global_pview := (restrict recLocs (view_to_zero CV)). *)
+(*     iMod (own_alloc (● (new_global_pview: viewUR) ⋅ ◯ _)) *)
+(*       as (new_pview_lb_name) "[globalPView globalPViewPts]". *)
+(*     { apply auth_both_valid. split; first done. apply view_valid. } *)
+(*     iDestruct "globalPViewPts" as "#globalPViewPts". *)
+
+(*     set newFullPreds := restrict recLocs predicates_full. *)
+(*     iMod (know_predicates_alloc newFullPreds) as *)
+(*       (new_full_predicates_name) "[newFullPreds #newFullPredsFrag]". *)
+(*     set newReadPreds := restrict recLocs predicates_read. *)
+(*     iMod (know_predicates_alloc newReadPreds) as *)
+(*       (new_read_predicates_name) "[newReadPreds #newReadPredsFrag]". *)
+(*     set newPersPreds := restrict recLocs predicates_pers. *)
+(*     iMod (know_predicates_alloc newPersPreds) as *)
+(*       (new_pers_predicates_name) "[newPersPreds #newPersPredsFrag]". *)
+
+(*     set newAtLocs := recLocs ∩ at_locs. *)
+(*     iMod (own_alloc (● (newAtLocs : gsetUR _) ⋅ ◯ _)) *)
+(*       as (new_shared_locs_name) "[newAtLocs atLocsFrag]". *)
+(*     { apply auth_both_valid. done. } *)
+(*     iDestruct "atLocsFrag" as "#atLocsFrag". *)
+
+(*     set newNaLocs := recLocs ∩ na_locs. *)
+(*     iMod (own_alloc (● (newNaLocs : gsetUR _) ⋅ ◯ _)) *)
+(*       as (new_exclusive_locs_name) "[newNaLocs naLocsFrag]". *)
+(*     { apply auth_both_valid. done. } *)
+(*     iDestruct "naLocsFrag" as "#naLocsFrag". *)
+
+(*     pose (newNaViews := gset_to_gmap (∅ : view) newNaLocs). *)
+(*     iMod (ghost_map_alloc newNaViews) as (new_na_views_name) "[naView naViewPts]". *)
+
+(*     iMod (ghost_map_alloc_persistent *)
+(*             (default 1%positive <$> slice_hist (MaxNat <$> newOffsets) abs_hists)) *)
+(*       as (new_crashed_in_name) "[crashedInAuth #crashedInPts]". *)
+(*     iMod (ghost_map_auth_persist with "crashedInAuth") as "#crashedInAuth". *)
+
+(*     (* Allocate the new map of bumpers. *) *)
+(*     set newBumpers := restrict recLocs bumpers. *)
+(*     iMod (own_all_bumpers_alloc newBumpers) *)
+(*          as (new_bumpers_name) "[newBumpers #bumpersFrag]". *)
+
+(*     set newPhysHists := *)
+(*       (λ (hist : gmap _ _), discard_msg_views <$> hist) <$> *)
+(*         (drop_all_above newOffsets phys_hists). *)
+(*     iMod (auth_map_map_alloc (A := leibnizO _) newPhysHists) *)
+(*       as (new_phys_hist_name) "[newPhysHists #newPhysHistFrag]". *)
+
+(*     (* We show a few results that will be useful below. *) *)
+(*     iAssert ( *)
+(*       □ ∀ `(AbstractState ST) ℓ (bumper : ST → ST), ⌜ is_Some (CV !! ℓ) ⌝ -∗ *)
+(*         own_know_bumper (get_bumpers_name hGD) ℓ bumper -∗ *)
+(*         ⌜ bumpers !! ℓ = Some _ ⌝ ∗ *)
+(*         own_know_bumper new_bumpers_name ℓ bumper)%I as "#bumperImpl". *)
+(*     { iIntros "!>" (???? ℓ bumper (t & cvLook)) "[mono pts]". *)
+(*       iFrame "mono". *)
+(*       iDestruct (ghost_map_lookup with "oldBumpers pts") as %bumpersLook. *)
+(*       iFrame (bumpersLook). *)
+(*       iApply (big_sepM_lookup with "bumpersFrag"). *)
+(*       apply restrict_lookup_Some. *)
+(*       split; first done. *)
+
+(*       apply elem_of_dom_2 in cvLook. *)
+(*       apply elem_of_dom_2 in bumpersLook. *)
+(*       apply elem_of_intersection. *)
+(*       rewrite domHistsEqBumpers. *)
+(*       split; done. } *)
+
+(*     iAssert ( *)
+(*       □ ∀ `(AbstractState ST) ℓ, *)
+(*         ⌜ is_Some (CV !! ℓ) ⌝ -∗ *)
+(*         know_preorder_loc ℓ (abs_state_relation (ST := ST)) -∗ *)
+(*         ⌜ orders !! ℓ = Some _ ⌝ ∗ *)
+(*         own_know_preorder_loc new_orders_name ℓ (abs_state_relation (ST := ST)))%I *)
+(*       as "#orderImpl". *)
+(*     { iIntros "!>" (???? ℓ (t & cvLook)) "order". *)
+(*       iDestruct (ghost_map_lookup with "allOrders order") as %ordersLook. *)
+(*       iFrame (ordersLook). *)
+(*       iApply (big_sepM_lookup with "fragOrders"). *)
+(*       apply restrict_lookup_Some. *)
+(*       split; first done. *)
+(*       apply elem_of_dom_2 in cvLook. *)
+(*       apply elem_of_dom_2 in ordersLook. *)
+(*       rewrite elem_of_intersection. *)
+(*       rewrite domHistsEqOrders. *)
+(*       split; done. } *)
+
+(*     (* The physical and abstract history has the same timestamps for all *) *)
+(* (*     locations. We will need this when we apply [valid_slice_transfer] below. *) *)
+(*     iAssert ( *)
+(*       ⌜∀ ℓ h1 h2, phys_hists !! ℓ = Some h1 → abs_hists !! ℓ = Some h2 → dom h1 = dom h2⌝ *)
+(*     )%I as %physAbsHistTimestamps. *)
+(*     { iIntros (?????). *)
+(*       iDestruct (big_sepM2_lookup with "predsFullHold") as (??) "(_ & sep)"; try eassumption. *)
+(*       iDestruct "sep" as "(_ & sep)". *)
+(*       iApply (big_sepM2_dom with "sep"). } *)
+
+(*     (* [CV] is a valid slice of the physical and abstract history. *) *)
+(*     assert (valid_slice CV (map_zip_with drop_prefix phys_hists offsets)) *)
+(*       as cvSlicesPhysHists. *)
+(*     { apply consistent_cut_valid_slice in cut. *)
+(*       eapply valid_slice_mono_l in cut; last apply physHistsSubStore. *)
+(*       done. } *)
+(*     assert (valid_slice (MaxNat <$> offsets_add offsets CV) abs_hists) as cvSlicesAbsHists. *)
+(*     { apply valid_slice_drop_prefix in cvSlicesPhysHists. *)
+(*       eapply valid_slice_transfer; done. } *)
+
+(*     (* We are done allocating ghost state and can now present a new bundle of *) *)
+(* (*     ghost names. *) *)
+(*     iModIntro. *)
+(*     set (hD' := {| *)
+(*       abs_history_name := new_abs_history_name; *)
+(*       phys_history_name := new_phys_hist_name; *)
+(*       non_atomic_views_gname := new_na_views_name; *)
+(*       crashed_in_name := new_crashed_in_name; *)
+(*       full_predicates_name := new_full_predicates_name; *)
+(*       read_predicates_name := new_read_predicates_name; *)
+(*       pers_predicates_name := new_pers_predicates_name; *)
+(*       preorders_name := new_orders_name; *)
+(*       offset_name := new_offset_name; *)
+(*       exclusive_locs_name := new_exclusive_locs_name; *)
+(*       shared_locs_name := new_shared_locs_name; *)
+(*       bumpers_name := new_bumpers_name; *)
+(*       pview_lb_name := new_pview_lb_name; *)
+(*     |}). *)
+(*     iExists (NvmDeltaG hGD' hD'). *)
+
+(*     assert (newNaLocs ## newAtLocs) as newLocsDisjoint. *)
+(*     { rewrite /newNaLocs /newAtLocs. set_solver+ locsDisjoint. } *)
+(*     assert (dom newAbsHists = newNaLocs ∪ newAtLocs) as newHistDomLocs. *)
+(*     { rewrite /newAbsHists /newNaLocs /newAtLocs /recLocs. *)
+(*       rewrite -domNewAbsHists. *)
+(*       rewrite /recLocs. *)
+(*       rewrite histDomLocs. *)
+(*       set_solver+. } *)
+(*     assert (newAbsHists = restrict newNaLocs newAbsHists ∪ *)
+(*                           restrict newAtLocs newAbsHists) as split. *)
+(*     { apply restrict_disjoint_union. done. } *)
+(*     iEval (rewrite split) in "knowHistories". *)
+(*     rewrite big_sepM_union. *)
+(*     2: { apply restrict_disjoint. done. } *)
+(*     iDestruct "knowHistories" as "[naHistories atHistories]". *)
+
+(*     iFrame "baseInterp". *)
+(*     rewrite /nvm_heap_ctx. rewrite /post_crash. *)
+(*     iDestruct ("P" $! _ (restrict na_locs abs_hists) bumpers na_views store _ *)
+(*                 with "persImpl baseMap") as "(baseMap & P)". *)
+(*     iDestruct *)
+(*       (map_points_to_to_new _ _ _ _ hGD' *)
+(*          with "newCrashedAt baseMap ptsMap") as "[baseMap ptsMap]"; first done. *)
+
+(*     iAssert ( *)
+(*       post_crash_resource_persistent hGD {| nvm_delta_base := hGD'; nvm_delta_high := hD' |} *)
+(*     ) as "#pcResPers". *)
+(*     { iSplit. *)
+(*       { (* We show that fragments of the histories may survive a crash. *) *)
+(*         iModIntro. *)
+(*         iIntros (???? ℓ t offset s bumper) "order oldOffset oldBumper frag". *)
+(*         iApply "orLost". iIntros (tC look). *)
+
+(*         iDestruct "frag" as (encX decEq) "oldFrag". *)
+
+(*         iDestruct ("bumperImpl" $! ST with "[//] oldBumper") *)
+(*           as "[%bumpersLook newBumper]". *)
+(*         iDestruct ("orderImpl" $! ST with "[//] order") *)
+(*           as "[%ordersLook newOrder]". *)
+(*         iDestruct (ghost_map_lookup with "oldOffsets oldOffset") as %offsetsLook. *)
+
+(*         assert (newOffsets !! ℓ = Some (offset + tC)) as newOffsetsLook. *)
+(*         { rewrite /newOffsets. *)
+(*           apply map_lookup_zip_with_Some. *)
+(*           eexists _, (MaxNat _). *)
+(*           split_and!; done. } *)
+
+(*         assert (ℓ ∈ recLocs). *)
+(*         { rewrite /recLocs. *)
+(*           rewrite domHistsEqOrders. *)
+(*           apply elem_of_intersection. *)
+(*           split; apply elem_of_dom; done. } *)
+
+(*         iDestruct (big_sepM_lookup _ _ ℓ with "offsetPts") as "offset". *)
+(*         { rewrite /newOffsets. *)
+(*           apply map_lookup_zip_with_Some. *)
+(*           eexists _, (MaxNat _). *)
+(*           split_and!; done. } *)
+
+(*         iDestruct (full_map_frag_entry with "oldFullHist oldFrag") *)
+(*           as %(oldAbsHist & lookH & hLook). *)
+
+(*         eassert _ as newHistLook. { apply new_abs_hist_lookup; done. } *)
+
+(*         eassert (is_Some (oldAbsHist !! (offset + tC))) as [sOld oldAbsHistLook]. *)
+(*         { eapply valid_slice_lookup; try done. *)
+(*           rewrite lookup_fmap. rewrite /offsets_add. *)
+(*           rewrite map_lookup_zip_with. *)
+(*           rewrite look. rewrite offsetsLook. simpl. *)
+(*           done. } *)
+
+(*         (* TODO: Make this a lemma. *) *)
+(*         iDestruct (big_sepM2_lookup with "bumperSome") *)
+(*           as %bumperSome; [done|done|]. *)
+(*         eassert _ as applyBumper. *)
+(*         { eapply map_Forall_lookup_1. *)
+(*           apply bumperSome. *)
+(*           apply oldAbsHistLook. } *)
+(*         destruct applyBumper as (? & temp). *)
+(*         assert _ as encodeBumper by apply temp. *)
+(*         apply encode_bumper_Some_decode in temp as (recS & decEq2 & <-). *)
+
+(*         assert (is_Some (phys_hists !! ℓ)) as [physHist physHistsLook]. *)
+(*         { rewrite -elem_of_dom domPhysHistsEqAbsHists elem_of_dom. done. } *)
+
+(*         eassert (is_Some (physHist !! _)) as [msg physHistLook]. *)
+(*         { apply elem_of_dom. *)
+(*           erewrite physAbsHistTimestamps; [ | done | done]. *)
+(*           apply elem_of_dom. *)
+(*           done. } *)
+
+(*         eassert _ as applyBumper. *)
+(*         { eapply map_Forall_lookup_1. *)
+(*           apply bumperSome. *)
+(*           apply hLook. } *)
+(*         destruct applyBumper as (? & temp). *)
+(*         assert _ as encodeBumper2 by apply temp. *)
+(*         apply encode_bumper_Some_decode in temp as (? & decEq' & <-). *)
+(*         simplify_eq. *)
+
+(*         iExists _, _. *)
+
+(*         iDestruct (big_sepM_lookup with "crashedInPts") as "#crashedIn". *)
+(*         { rewrite lookup_fmap. *)
+(*           erewrite slice_hist_lookup_Some; try done. *)
+(*           rewrite lookup_fmap. *)
+(*           erewrite newOffsetsLook. *)
+(*           done. } *)
+
+(*         iSplit. *)
+(*         { iExists sOld. iFrame "crashedIn". iPureIntro. apply decEq2. } *)
+(*         iAssert (frag_entry_unenc new_abs_history_name ℓ (offset + tC) (bumper recS))%I as "#frag". *)
+(*         { iDestruct (big_sepM_lookup with "fragHistories") as "HI"; try done. *)
+(*           iDestruct (big_sepM_lookup with "HI") as "HI2"; try done. *)
+(*           { rewrite /new_hist. *)
+(*             rewrite lookup_omap. *)
+(*             erewrite drop_above_lookup_t. *)
+(*             rewrite oldAbsHistLook /=. *)
+(*             rewrite encodeBumper. *)
+(*             done. } *)
+(*           rewrite /know_frag_history_loc. *)
+(*           rewrite /frag_entry_unenc. *)
+(*           iExists _. *)
+(*           iFrame "HI2". *)
+(*           rewrite decode_encode. done. } *)
+(*         iFrameF "frag". *)
+
+(*         iDestruct (auth_map_map_frag_lookup_singleton with "newPhysHistFrag") as "$". *)
+(*         { rewrite /newPhysHists. rewrite lookup_fmap. rewrite /drop_all_above. *)
+(*           rewrite map_lookup_zip_with. *)
+(*           rewrite newOffsetsLook /=. rewrite physHistsLook /=. *)
+(*           done. } *)
+(*         { rewrite lookup_fmap drop_above_lookup_t physHistLook. done. } *)
+
+(*         iIntros ([lt | ->]%Nat.lt_eq_cases). *)
+(*         2: { assert (s = recS) as -> by congruence. iFrame "frag". done. } *)
+
+(*         iDestruct (big_sepM_lookup with "fragHistories") as "HI"; try done. *)
+(*         iDestruct (big_sepM_lookup with "HI") as "HI2"; try done. *)
+(*         { rewrite /new_hist. *)
+(*           rewrite lookup_omap. *)
+(*           erewrite drop_above_lookup_le; last (apply Nat.lt_le_incl; apply lt). *)
+(*           rewrite hLook. *)
+(*           simpl. *)
+(*           rewrite encodeBumper2. *)
+(*           done. } *)
+(*         iDestruct (big_sepM2_lookup with "ordered") as %incr; try done. *)
+(*         iSplitPure. *)
+(*         { eapply encode_relation.encode_relation_decode_iff_1; try done. *)
+(*           eapply incr; done. } *)
+(*         iExists _. *)
+(*         iFrame "HI2". *)
+(*         rewrite decode_encode. *)
+(*         done. } *)
+
+(*       (* The preorder implication. We show that the preorders may survive a *) *)
+(* (*         crash. *) *)
+(*       iSplit. *)
+(*       { iModIntro. *)
+(*         iIntros (? ? ? ? ?) "order". *)
+(*         iApply "orLost". iIntros (t look). *)
+(*         iDestruct ("orderImpl" $! ST with "[//] order") as "[_ $]". } *)
+
+(*       (* "post_crash_full_pred_impl" - We show that the predicates survives a *) *)
+(* (*       crash. *) *)
+(*       iSplitL "". *)
+(*       { rewrite /post_crash_full_pred_impl. *)
+(*         iModIntro. *)
+(*         iIntros (??? ℓ ϕ) "oldFullPred". *)
+(*         iApply "orLost". iIntros (t look). *)
+(*         iDestruct (own_all_preds_pred with "allFullPredicates oldFullPred") *)
+(*           as (encPred predsLook) "#equiv". *)
+(*         iNext. *)
+(*         rewrite /know_pred. *)
+(*         iDestruct (predicates_frag_lookup with "newFullPredsFrag") as "newFullPred". *)
+(*         { rewrite /newFullPreds. *)
+(*           apply restrict_lookup_Some. *)
+(*           split; try done. *)
+(*           apply elem_of_dom_2 in look. *)
+(*           apply elem_of_dom_2 in predsLook. *)
+(*           rewrite /recLocs. *)
+(*           rewrite domHistsEqBumpers -FullBumperDoms. *)
+(*           set_solver+ look predsLook. } *)
+(*         rewrite /full_predicates_name. simpl. *)
+(*         iApply ( *)
+(*           internal_eq_rewrite _ _ *)
+(*             (λ (r : enc_predicateO), *)
+(*               own new_full_predicates_name (◯ {[ℓ := pred_to_ra r]})) with "equiv"); *)
+(*           last done. *)
+(*         solve_proper. } *)
+(*       (* "post_crash_read_pred_impl" - We show that the predicates survives a *) *)
+(* (*       crash. *) *)
+(*       iSplitL "". *)
+(*       { rewrite /post_crash_read_pred_impl. *)
+(*         iModIntro. *)
+(*         iIntros (??? ℓ ϕ) "oldReadPred". *)
+(*         iApply "orLost". iIntros (t look). *)
+(*         iDestruct (own_all_preds_pred with "allReadPredicates oldReadPred") *)
+(*           as (encPred predsLook) "#equiv". *)
+(*         iNext. *)
+(*         rewrite /know_pred. *)
+(*         iDestruct (predicates_frag_lookup with "newReadPredsFrag") as "newReadPred". *)
+(*         { rewrite /newReadPreds. *)
+(*           apply restrict_lookup_Some. *)
+(*           split; try done. *)
+(*           apply elem_of_dom_2 in look. *)
+(*           apply elem_of_dom_2 in predsLook. *)
+(*           rewrite /recLocs. *)
+(*           rewrite domHistsEqBumpers -ReadBumperDoms. *)
+(*           set_solver+ look predsLook. } *)
+(*         rewrite /read_predicates_name. simpl. *)
+(*         iApply ( *)
+(*           internal_eq_rewrite _ _ *)
+(*             (λ (r : enc_predicateO), *)
+(*               own new_read_predicates_name (◯ {[ℓ := pred_to_ra r]})) with "equiv"); *)
+(*           last done. *)
+(*         solve_proper. } *)
+(*       (* "post_crash_pers_pred_impl" - We show that the predicates survives a *) *)
+(* (*       crash. *) *)
+(*       iSplitL "". *)
+(*       { rewrite /post_crash_pers_pred_impl. *)
+(*         iModIntro. *)
+(*         iIntros (??? ℓ ϕ) "oldPersPred". *)
+(*         iApply "orLost". iIntros (t look). *)
+(*         iDestruct (own_all_preds_pred with "allPersPredicates oldPersPred") *)
+(*           as (encPred predsLook) "#equiv". *)
+(*         iNext. *)
+(*         rewrite /know_pred. *)
+(*         iDestruct (predicates_frag_lookup with "newPersPredsFrag") as "newPersPred". *)
+(*         { rewrite /newPersPreds. *)
+(*           apply restrict_lookup_Some. *)
+(*           split; try done. *)
+(*           apply elem_of_dom_2 in look. *)
+(*           apply elem_of_dom_2 in predsLook. *)
+(*           rewrite /recLocs. *)
+(*           rewrite domHistsEqBumpers -PersBumperDoms. *)
+(*           set_solver+ look predsLook. } *)
+(*         rewrite /pers_predicates_name. simpl. *)
+(*         iApply ( *)
+(*           internal_eq_rewrite _ _ *)
+(*             (λ (r : enc_predicateO), *)
+(*               own new_pers_predicates_name (◯ {[ℓ := pred_to_ra r]})) with "equiv"); *)
+(*           last done. *)
+(*         solve_proper. } *)
+(*       (* "post_crash_at_loc_impl" - Shared locations. *) *)
+(*       iSplit. { *)
+(*         rewrite /post_crash_at_loc_impl. *)
+(*         iIntros "!>" (ℓ) "sh". *)
+(*         iApply "orLost". iIntros (t look). *)
+(*         iDestruct (own_valid_2 with "atLocs sh") *)
+(*           as %[_ [elem _]]%auth_both_dfrac_valid_discrete. *)
+(*         iApply (own_mono with "atLocsFrag"). *)
+(*         exists (◯ newAtLocs). *)
+(*         rewrite -auth_frag_op. *)
+(*         rewrite gset_op. *)
+(*         f_equiv. *)
+(*         apply gset_included in elem. *)
+(*         symmetry. *)
+(*         eapply subseteq_union_1. *)
+(*         rewrite /newAtLocs. *)
+(*         apply elem_of_subseteq_singleton. *)
+(*         apply elem_of_intersection. *)
+(*         split; last set_solver. *)
+(*         rewrite /newAbsHists. *)
+(*         apply elem_of_intersection. *)
+(*         split; last first. *)
+(*         { rewrite histDomLocs. set_solver+ elem. } *)
+(*         apply elem_of_dom. *)
+(*         naive_solver. } *)
+(*       iSplit. { *)
+(*         rewrite /post_crash_na_loc_impl. *)
+(*         iIntros "!>" (ℓ) "sh". *)
+(*         iApply "orLost". iIntros (t look). *)
+(*         iDestruct (own_valid_2 with "naLocs sh") *)
+(*           as %[_ [elem _]]%auth_both_dfrac_valid_discrete. *)
+(*         iApply (own_mono with "naLocsFrag"). *)
+(*         exists (◯ newNaLocs). *)
+(*         rewrite -auth_frag_op. *)
+(*         rewrite gset_op. *)
+(*         f_equiv. *)
+(*         apply gset_included in elem. *)
+(*         symmetry. *)
+(*         eapply subseteq_union_1. *)
+(*         rewrite /newNaLocs. *)
+(*         apply elem_of_subseteq_singleton. *)
+(*         apply elem_of_intersection. *)
+(*         split; last set_solver + elem. *)
+(*         apply elem_of_dom_2 in look. *)
+(*         set_solver+ look histDomLocs elem. } *)
+(*       (* "post_crash_offsets_impl" *) *)
+(*       iSplit. { *)
+(*         rewrite /offsets_impl. *)
+(*         iIntros "!>" (ℓ oldOffset) "oldOffset". *)
+(*         iApply "orLost". iIntros (t cvLook). *)
+(*         iDestruct (ghost_map_lookup with "oldOffsets oldOffset") as %look. *)
+(*         iApply (big_sepM_lookup with "offsetPts"). *)
+(*         rewrite /newOffsets. *)
+(*         apply map_lookup_zip_with_Some. *)
+(*         eexists _, (MaxNat _). *)
+(*         split; first reflexivity. *)
+(*         split; done. } *)
+(*       (* "post_crash_bumper_impl" *) *)
+(*       { iIntros "!>" (? ? ? ? ℓ bumper) "oldBumper". *)
+(*         iApply "orLost". iIntros (t cvLook). *)
+(*         iDestruct ("bumperImpl" $! ST with "[//] oldBumper") *)
+(*           as "[%bumpersLook newBumper]". *)
+(*         iFrame "newBumper". } } *)
+
+(*     (* We show the assumption for the post crash modality. *) *)
+(*     iDestruct ("P" with "[atLocsHistories naHistories naViewPts]") as "[$ pcRes]". *)
+(*     { rewrite /post_crash_resource. *)
+(*       iFrame "pcResPers". *)
+(*       (* "post_crash_na_view_map" *) *)
+(*       iSplitL "naViewPts". *)
+(*       { rewrite /post_crash_na_view_map. *)
+(*         iSplitL "". *)
+(*         { iIntros (ℓ q SV). iApply (ghost_map_lookup with "oldNaView"). } *)
+(*         iDestruct (big_sepM_impl_strong with "naViewPts []") as "[$ H]". *)
+(*         iIntros "!>" (ℓ V). *)
+(*         destruct (newNaViews !! ℓ) as [newV|] eqn:eq. *)
+(*         - iIntros "newPts look". *)
+(*           rewrite /newNaViews in eq. *)
+(*           apply lookup_gset_to_gmap_Some in eq as [hup <-]. *)
+(*           iApply soft_disj_intro_r. *)
+(*           iApply "orLost". iIntros (t look). *)
+(*           iApply "newPts". *)
+(*         - iIntros "_ %naViewsLook". *)
+(*           iApply soft_disj_intro_r. *)
+(*           iExists _. iFrame "newCrashedAt". *)
+(*           iRight. iPureIntro. *)
+(*           move: eq. *)
+(*           rewrite /newNaViews. *)
+(*           rewrite lookup_gset_to_gmap_None. *)
+(*           rewrite /newNaLocs. *)
+(*           rewrite not_elem_of_intersection. *)
+(*           intros [elem|elem]. *)
+(*           2: { exfalso. apply elem. rewrite -naViewsDom. eapply elem_of_dom_2. *)
+(*                apply naViewsLook. } *)
+(*           rewrite /recLocs in elem. *)
+(*           apply not_elem_of_dom. *)
+(*           apply elem_of_dom_2 in naViewsLook. *)
+(*           rewrite histDomLocs in elem. *)
+(*           rewrite naViewsDom in naViewsLook. *)
+(*           set_solver+ elem naViewsLook. } *)
+(*       (* "post_crash_full_history_map" *) *)
+(*       rewrite /post_crash_full_history_map. *)
+(*       iSplitL "atLocsHistories". *)
+(*       { iIntros (ℓ q hist) "hist". *)
+(*         iDestruct (full_map_full_entry with "oldFullHist hist") as %look. *)
+(*         destruct (decide (ℓ ∈ at_locs)) as [?|notElem]. *)
+(*         { iDestruct (big_sepM_lookup with "atLocsHistories") as "H". *)
+(*           { apply restrict_lookup_Some; done. } *)
+(*           iCombine "H hist" as "H2". *)
+(*           iDestruct (full_entry_valid with "H2") as %val. *)
+(*           iPureIntro. exfalso. *)
+(*           apply (Qp.not_add_le_l 1 q). *)
+(*           apply val. } *)
+(*         iPureIntro. *)
+(*         apply restrict_lookup_Some. *)
+(*         split; first done. *)
+(*         apply elem_of_dom_2 in look. *)
+(*         set_solver+ notElem histDomLocs look. } *)
+(*       iSplitL "". *)
+(*       { iIntros (ℓ bumper). iApply (ghost_map_lookup with "oldBumpers"). } *)
+(*       iDestruct (big_sepM_impl_strong with "naHistories []") as "[$ H]". *)
+(*       iIntros "!>" (ℓ oldAbsHist) "pts". *)
+(*       iIntros ([absHistLook elem]%restrict_lookup_Some). *)
+(*       assert (is_Some (bumpers !! ℓ)) as [bumper ?]. *)
+(*       { apply elem_of_dom. *)
+(*         rewrite -domHistsEqBumpers. *)
+(*         apply elem_of_dom. *)
+(*         eexists _. apply absHistLook. } *)
+(*       assert (is_Some (offsets !! ℓ)) as [offset ?]. *)
+(*       { apply elem_of_dom. *)
+(*         rewrite -offsetDom domPhysHistsEqAbsHists. *)
+(*         apply elem_of_dom. *)
+(*         eexists _. apply absHistLook. } *)
+(*       assert (is_Some (phys_hists !! ℓ)) as [physHist physHistsLook]. *)
+(*       { rewrite -elem_of_dom domPhysHistsEqAbsHists elem_of_dom. done. } *)
+(*       iExists bumper. iSplitPure; first done. *)
+(*       iApply soft_disj_intro_r. *)
+(*       iApply "orLost". iIntros (tC cvLook). *)
+(*       assert (newOffsets !! ℓ = Some (offset + tC)) as newOffsetsLook. *)
+(*       { rewrite /newOffsets. *)
+(*         apply map_lookup_zip_with_Some. *)
+(*         eexists _, (MaxNat _). *)
+(*         split_and!; done. } *)
+
+(*       rewrite restrict_lookup_elem_of. *)
+(*       2: { rewrite /newNaLocs. *)
+(*         apply elem_of_dom_2 in cvLook. *)
+(*         apply elem_of_dom_2 in absHistLook. *)
+(*         set_solver+ elem cvLook absHistLook. } *)
+(*       eassert (new_abs_hist abs_hists newOffsets bumpers !! ℓ = Some _) *)
+(*         as newAbsHistLook. *)
+(*       { apply map_lookup_zip_with_Some. *)
+(*         eexists _, _. *)
+(*         split_and!; try done. *)
+(*         rewrite /drop_all_above. *)
+(*         apply map_lookup_zip_with_Some. *)
+(*         eexists _, _. *)
+(*         split_and!; done. } *)
+(*       rewrite newAbsHistLook. *)
+(*       eassert (is_Some (oldAbsHist !! (offset + tC))) as [sOld ?]. *)
+(*       { eapply valid_slice_lookup; try done. *)
+(*         rewrite lookup_fmap. rewrite /offsets_add. *)
+(*         rewrite map_lookup_zip_with. *)
+(*         rewrite cvLook. rewrite H1. simpl. *)
+(*         done. } *)
+(*       eassert (is_Some (physHist !! _)) as [msg physHistLook]. *)
+(*       { apply elem_of_dom. *)
+(*         erewrite physAbsHistTimestamps; [ | done | done]. *)
+(*         apply elem_of_dom. *)
+(*         done. } *)
+(*       iDestruct (big_sepM2_lookup with "bumperSome") as %bv; [done|done|]. *)
+(*       eassert _ as temp. *)
+(*       { eapply map_Forall_lookup_1; [eapply bv|done]. } *)
+(*       destruct temp as [sNew ?]. *)
+(*       iExists _, sOld, _, msg.(msg_val). *)
+(*       iDestruct (big_sepM_lookup with "offsetPts") as "$"; first done. *)
+(*       iSplitPure; first done. *)
+(*       iSplitPure; first done. *)
+(*       iSplit. *)
+(*       { iApply (big_sepM_lookup with "crashedInPts"). *)
+(*         rewrite lookup_fmap. *)
+(*         erewrite slice_hist_lookup_Some; try done. *)
+(*         rewrite lookup_fmap. *)
+(*         rewrite newOffsetsLook. *)
+(*         simpl. *)
+(*         f_equiv. } *)
+(*       iFrame "pts". *)
+(*       iDestruct (big_sepM_lookup with "fragHistories") as "frags"; first done. *)
+(*       (* Note: At this point we could easily give all the fractional entries. *) *)
+(*       iDestruct (big_sepM_lookup with "frags") as "$". *)
+(*       { apply lookup_omap_Some. eexists _. *)
+(*         split; first done. rewrite drop_above_lookup_t. done. } *)
+(*       iDestruct (auth_map_map_frag_lookup_singleton with "newPhysHistFrag") as "$". *)
+(*       { rewrite /newPhysHists. rewrite lookup_fmap. rewrite /drop_all_above. *)
+(*         rewrite map_lookup_zip_with. *)
+(*         rewrite newOffsetsLook /=. rewrite physHistsLook /=. *)
+(*         done. } *)
+(*       { rewrite lookup_fmap drop_above_lookup_t physHistLook. done. } *)
+(*     } *)
+(*     iFrame "valView". *)
+(*     iSplitPure. { subst. done. } *)
+(*     (* We show the state interpretation for the high-level logic. *) *)
+(*     iExistsN. *)
+(*     rewrite /full_map. *)
+
+(*     iFrame "offsets". *)
+(*     iFrame "newPhysHists". *)
+(*     rewrite /newPhysHists /newOffsets. *)
+
+(*     rewrite slice_of_store_drop. *)
+
+(*     iFrame "ptsMap". *)
+(*     (* iFrame "offsets". *) *)
+(*     iFrame "newOrders newFullPreds newReadPreds newPersPreds hists' newAtLocs newCrashedAt". *)
+(*     iFrame "newNaLocs". *)
+(*     (* iFrame "newPhysHists". *) *)
+(*     iFrame "newBumpers". *)
+(*     iFrame "naView". *)
+(*     iFrame "fragHistories". *)
+(*     (* [oldViewsDiscarded] *) *)
+(*     iSplit. *)
+(*     { (* Showing this is easy as we have indeed discarded all views. *) *)
+(*       iIntros "!>". iApply big_sepM2_forall. *)
+(*       iSplitPure. *)
+(*       { apply dom_eq_alt_L. *)
+(*         rewrite dom_fmap_L. *)
+(*         rewrite /offsets_add /drop_all_above !dom_map_zip_with_L. *)
+(*         rewrite -offsetDom. *)
+(*         set_solver+. } *)
+(*       iPureIntro. *)
+(*       intros ??? (? & ? & ?)%lookup_fmap_Some ???? look. *)
+(*       simplify_eq. *)
+(*       apply lookup_fmap_Some in look as (? & <- & ?). *)
+(*       done. } *)
+
+(*     (* GlobalPViewPersisted *) *)
+(*     iSplit. { *)
+(*       iPoseProof (persisted_weak _ new_global_pview with "[$]") as "$". *)
+(*       apply view_le_lookup. *)
+(*       intros. *)
+(*       exists t. split; last done. *)
+(*       by apply restrict_lookup_Some in H0 as [? ?]. *)
+(*     } *)
+
+(*     (* (* GlobalPView *) *) *)
+(*     (* iSplitL "globalPView"; first iFrame. *) *)
+(*     (* [locDisjoint] *) *)
+(*     iSplitPure. *)
+(*     { set_solver. } *)
+(*     (* [histDomLocs] *) *)
+(*     iSplitPure. { rewrite -domNewAbsHists. set_solver+ histDomLocs. } *)
+(*     (* [naView] *) *)
+(*     iSplitPure. { rewrite /newNaViews. apply dom_gset_to_gmap. } *)
+(*     (* mapShared. We show that the shared location still satisfy that *) *)
+(* (*     their two persist-views are equal. *) *)
+(*     iSplitPure. *)
+(*     { rewrite /shared_locs_inv. *)
+(*       rewrite /map_map_Forall. *)
+(*       eapply map_Forall_subseteq. { apply restrict_subseteq. } *)
+(*       intros ℓ hist look t newMsg histLook. *)
+(*       apply map_lookup_zip_with_Some in look as (hist' & off & -> & look & offsetsLook). *)
+(*       apply lookup_fmap_Some in look as (origHist & <- & look). *)
+(*       apply drop_all_above_lookup_Some in look as (? & ? & -> & ? & ?). *)
+(*       rewrite drop_above_fmap in histLook. *)
+(*       simplify_eq. *)
+(*       apply drop_prefix_drop_above in histLook as (-> & look). *)
+(*       apply lookup_fmap_Some in look as (? & <- & ? ). *)
+(*       split; last done. *)
+(*       destruct x1. simpl. apply view_lookup_zero_empty. } *)
+(*     (* atLocsHistories *) *)
+(*     iSplitL "atHistories". *)
+(*     { iNext. *)
+(*       iApply (big_sepM_impl with "atHistories"). *)
+(*       iIntros "!>" (ℓ ? [??]%restrict_lookup_Some) "$". } *)
+(*     (* [ordered]: We show that the abstract states are still ordered. *) *)
+(*     iSplitR. *)
+(*     { iApply big_sepM2_intro. *)
+(*       { setoid_rewrite <- elem_of_dom. *)
+(*         apply set_eq. *)
+(*         rewrite restrict_dom_subset_L; first done. *)
+(*         rewrite -domHistsEqOrders. *)
+(*         set_solver+. } *)
+(*       iModIntro. *)
+(*       iModIntro. *)
+(*       iIntros (ℓ newHist order ih [ordersLook ?]%restrict_lookup_Some). *)
+(*       apply new_abs_hist_lookup_Some in ih *)
+(*           as (bumper & hist & ? & ? & ? & ? & ?). *)
+(*       simplify_eq. *)
+(*       iDestruct (big_sepM2_lookup with "ordered") as %incr; [done|done| ]. *)
+(*       iDestruct (big_sepM2_lookup with "bumpMono") as %mono; [done|done| ]. *)
+(*       iPureIntro. *)
+
+(*       intros ?????. *)
+(*       intros (? & ? & [??]%map_filter_lookup_Some)%lookup_omap_Some *)
+(*              (? & ? & [??]%map_filter_lookup_Some)%lookup_omap_Some. *)
+(*       eapply mono; [done | done |]. *)
+(*       eapply incr; [ |done|done]. *)
+(*       lia. } *)
+
+(*     (* histPViewDoms *) *)
+(*     iSplit. { *)
+(*       iPureIntro. *)
+(*       rewrite -domNewAbsHists. *)
+(*       rewrite restrict_dom_subset_L; first done. *)
+(*       set_solver. *)
+(*     } *)
+
+(*     (* for the recovery of the triple predicates, we need to process at once: *) *)
+(* (*        for each location, we need both the resource from [full] and [pers] to *) *)
+(* (*        invoke the [predsPostCrash] condition. *) *)
+
+(*     (* gathering hypotheses *) *)
+(*     iPoseProof (big_sepM2_sep_2 with "predsReadHold predsPersHold") as "predsHold". *)
+(*     iPoseProof (big_sepM2_sep_2 with "predsFullHold predsHold") as "predsHold". *)
+(*     rewrite [named "predsFullHold" _]/named [named "predsReadHold" _]/named [named "predsPersHold" _]/named. *)
+(*     rewrite bi.sep_assoc -big_sepM2_sep. *)
+(*     rewrite bi.sep_assoc -big_sepM2_sep. *)
+(*     (* now we can split the goal properly, and show that the encoded predicates *) *)
+(* (*        still holds for the new abstract history *) *)
+
+(*     iSplitL "baseMap pcRes predsHold". *)
+(*     { *)
+(*       iApply big_sepM2_later_2. *)
+(*       iDestruct (big_sepM2_impl_dom_subseteq_with_resource with "[baseMap pcRes] predsHold [#]") as "[? $]". *)
+(*       { rewrite dom_fmap_L. *)
+(*         rewrite /drop_all_above /offsets_add !dom_map_zip_with_L. *)
+(*         set_solver+. } *)
+(*       { rewrite -domNewAbsHists. *)
+(*         rewrite dom_fmap_L. *)
+(*         rewrite /drop_all_above /offsets_add !dom_map_zip_with_L. *)
+(*         rewrite /recLocs. *)
+(*         rewrite -domPhysHistsEqAbsHists. *)
+(*         rewrite -offsetDom. *)
+(*         set_solver+. } *)
+(*       { iAccu. } *)
+
+(*       iModIntro. *)
+(*       iIntros (ℓ physHist absHist newPhysHist newAbsHist physHistsLook *)
+(*                absHistsLook newPhysHistsLook newAbsHistLook). *)
+(*       iIntros "[baseMap pcRes]". *)
+
+(*       (* (* Infer what we can from the lookup in the new physical history. *) *) *)
+(*       apply lookup_fmap_Some in newPhysHistsLook as (? & ? & look). *)
+(*       apply drop_all_above_lookup_Some in look as (newOffset & ? & -> & newOffsetLook & ?). *)
+(*       simplify_eq. *)
+(*       eassert _ as eq by apply newOffsetLook. *)
+(*       apply map_lookup_zip_with_Some in eq as (oldOffset & [tC] &?&?& cvLook). *)
+
+(*       (* Infer what we can from the lookup in the new abstract history. *) *)
+(*       apply new_abs_hist_lookup_Some in newAbsHistLook *)
+(*         as (bumper & ? & ? & offsetLook & ? & ? & bumpersLook). *)
+(*       rewrite /newOffsets in offsetLook. *)
+(*       simplify_eq. *)
+
+(*       iIntros "((%predFull & % & %predsFullLook & % & fullEncs) & *)
+(*                 (%predRead & % & %predsReadLook & % & readEncs) & *)
+(*                 (%predPers & %old_ts & %old_pers_encS & %old_pers_msg & *)
+(*                  %predsPersLook & %globalPViewLook & %absHistPersLook & *)
+(*                  %physHistPersLook & persEnc))". *)
+(*       simplify_eq. *)
+
+(*       distrib_later. *)
+(*       pull_left (▷ (∃ _ _, ⌜newFullPreds !! _ = _⌝ ∗ _))%I. *)
+
+(*       set (tCrash := oldOffset + tC). *)
+(*       (* predsFull *) *)
+(*       rewrite bi.later_exist bi.sep_exist_r. *)
+(*       iExists predFull. *)
+(*       rewrite bi.later_exist bi.sep_exist_r. *)
+
+(*       iExists (tCrash). *)
+(*       iAssert (⌜newFullPreds !! ℓ = Some predFull⌝)%I as "$". { *)
+(*         iPureIntro. *)
+(*         rewrite /newFullPreds. *)
+(*         apply restrict_lookup_Some_2; first done. *)
+(*         apply elem_of_dom_2 in cvLook. *)
+(*         apply elem_of_dom_2 in absHistsLook. *)
+(*         set_solver+ cvLook absHistsLook. } *)
+(*       rewrite bi.later_sep -bi.sep_assoc. *)
+(*       iSplitPure; first done. *)
+(*       (* predsRead *) *)
+(*       pull_left (▷ (∃ _ _, ⌜newReadPreds !! _ = _⌝ ∗ _))%I. *)
+(*       rewrite bi.later_exist bi.sep_exist_r. *)
+(*       iExists predRead. *)
+(*       rewrite bi.later_exist bi.sep_exist_r. *)
+(*       iExists (tCrash). *)
+(*       iAssert (⌜newReadPreds !! ℓ = Some predRead⌝)%I as "$". { *)
+(*         iPureIntro. *)
+(*         rewrite /newReadPreds. *)
+(*         apply restrict_lookup_Some_2; first done. *)
+(*         apply elem_of_dom_2 in cvLook. *)
+(*         apply elem_of_dom_2 in absHistsLook. *)
+(*         set_solver+ cvLook absHistsLook. } *)
+(*       rewrite bi.later_sep -bi.sep_assoc. *)
+(*       iSplitPure; first done. *)
+
+(*       (* predsPers *) *)
+(*       pull_left (▷ (∃ _ _ _ _, _))%I. *)
+(*       rewrite bi.later_exist bi.sep_exist_r. *)
+(*       iExists predPers. *)
+(*       rewrite bi.later_exist bi.sep_exist_r. *)
+(*       iExists (tCrash). *)
+(*       rewrite bi.later_exist bi.sep_exist_r. *)
+(*       (* obtains the encoded state through valid_slice *) *)
+(*       iAssert (∃ encS, ⌜ omap bumper (drop_above (tCrash) absHist)!! *)
+(*                       (tCrash)%nat = Some encS ⌝)%I *)
+(*         as (new_encS) "%". { *)
+(*         apply (slice_hist_Some _ _ ℓ (tCrash) absHist) *)
+(*           in cvSlicesAbsHists as (encS & absHistLook & ?); *)
+(*           [ | | done ]. *)
+(*         2: { *)
+(*           rewrite lookup_fmap_Some. *)
+(*           eexists. *)
+(*           split; done. *)
+(*         } *)
+(*         iPoseProof (big_sepM2_lookup_acc with "bumperSome") *)
+(*           as "[%bumperLook _]"; *)
+(*           [exact absHistsLook | exact bumpersLook | ]. *)
+(*         iPureIntro. *)
+(*         pose proof (map_Forall_lookup_1 _ _ _ _ bumperLook absHistLook) *)
+(*           as [encS' ?]. *)
+(*         rewrite map_Forall_lookup /is_Some in bumperLook. *)
+(*         eexists. *)
+(*         rewrite lookup_omap_Some. *)
+(*         eexists. *)
+(*         rewrite drop_above_lookup_t. *)
+(*         done. *)
+(*       } *)
+(*       iExists new_encS. *)
+(*       (* for some reason, [bi.later_exist] fail with typeclasses... *) *)
+(*       rewrite -bi.later_exist_2 bi.sep_exist_r. *)
+(*       assert (∃ msg, (drop_above (tCrash) physHist) !! (tCrash)%nat = Some msg) *)
+(*         as [new_msg newMsgLook]. { *)
+(*         pose proof (slice_hist_Some _ _ ℓ tC (drop_prefix physHist oldOffset) *)
+(*                       cvSlicesPhysHists *)
+(*                       ltac:(done) *)
+(*                       ltac:(rewrite map_lookup_zip_with_Some; *)
+(*                             eexists _, _; done)) as [msg [physHistLook _]]. *)
+(*         rewrite drop_prefix_lookup in physHistLook. rewrite Nat.add_comm in physHistLook. *)
+(*         eexists. *)
+(*         rewrite drop_above_lookup_t. *)
+(*         done. *)
+(*       } *)
+(*       iExists (discard_msg_views new_msg). *)
+(*       iAssert (⌜newPersPreds !! ℓ = Some predPers⌝)%I as "$". *)
+(*       { iPureIntro. *)
+(*         rewrite /newPersPreds. *)
+(*         apply restrict_lookup_Some_2; first done. *)
+(*         apply elem_of_dom_2 in cvLook. *)
+(*         apply elem_of_dom_2 in absHistsLook. *)
+(*         set_solver+ cvLook absHistsLook. } *)
+
+(*       (* [iFrame "%"] takes too long on my computer, *) *)
+(* (*          therefore I'm refactoring the goal here *) *)
+(*       do ? lazymatch goal with *)
+(*              | |- context [ ((_ ∗ _) ∗ _)%I ] => rewrite -bi.sep_assoc *)
+(*              | |- context [ (▷ (_ ∗ _))%I ] => rewrite bi.later_sep *)
+(*              end. *)
+
+(*       iSplitPure. { *)
+(*         left. *)
+(*         rewrite /offsets_add. *)
+(*         rewrite map_lookup_zip_with_Some. *)
+(*         eexists. exists (MaxNat 0). *)
+(*         split; first done. *)
+(*         split. *)
+(*         - rewrite map_lookup_zip_with_Some. *)
+(*           exists oldOffset, (MaxNat tC). *)
+(*           done. *)
+(*         - rewrite restrict_lookup_Some. *)
+(*           rewrite (view_to_zero_lookup _ _ (MaxNat tC)); last done. *)
+(*           split; first done. *)
+(*           rewrite elem_of_intersection. *)
+(*           split; eapply elem_of_dom_2; done. *)
+(*       } *)
+(*       iSplitPure; first done. *)
+(*       iSplitPure; first by (rewrite lookup_fmap_Some; eexists). *)
+
+(*       iDestruct (big_sepM2_dom with "fullEncs") as %physEncDomEq. *)
+(*       iDestruct (big_sepM2_lookup with "bumperSome") as %map; [done|done|]. *)
+
+(*       rewrite -2!big_sepM2_later_2. *)
+(*       pull_left ([∗ map] _↦ _; _ ∈ _; _, ▷ (_ -∗ ⌜ _ = None ⌝ -∗ _))%I. *)
+(*       iApply bi.wand_frame_r. { *)
+(*         iApply (big_sepM_singleton_hold _ _ _ (tCrash)); *)
+(*           [ | | by rewrite lookup_fmap_Some; eexists | done ]. *)
+(*         2: { *)
+(*           rewrite dom_fmap_L. *)
+(*           rewrite dom_omap_id_L; first by apply drop_above_dom_eq. *)
+(*           eapply (map_Forall_subseteq); first apply map_filter_subseteq. *)
+(*           apply map; done. *)
+(*         } *)
+(*         rewrite dom_fmap_L. *)
+(*         iIntros (???? elemOf) "_". iModIntro. iIntros. *)
+(*         rewrite elem_of_dom in elemOf. *)
+(*         rewrite drop_above_lookup_gt in elemOf; last by lia. *)
+(*         apply is_Some_None in elemOf. *)
+(*         done. *)
+(*       } *)
+(*       iSimpl. *)
+
+(*       rewrite -2!bi_wand_drop_premise. *)
+
+(*       assert (default ∅ (newNaViews !! ℓ) = ∅) as ->. { *)
+(*         rewrite /newNaViews. *)
+(*         destruct (gset_to_gmap ∅ newNaLocs !! ℓ) eqn:eq. *)
+(*         - apply lookup_gset_to_gmap_Some in eq as [_ ->]. done. *)
+(*         - done. *)
+(*       } *)
+
+(*       (* calculate the state for maximal timestamp (the full timestamp we will use) *) *)
+(*       set t_full := max_msg physHist. *)
+(*       assert (is_Some $ physHist !! t_full) as [full_msg physHistFullLook]. { *)
+(*         apply elem_of_dom. *)
+(*         rewrite /max_msg. *)
+(*         apply elem_of_elements. *)
+(*         apply max_list_elem_of. *)
+(*         apply elem_of_dom_2 in physHistPersLook. *)
+(*         apply elem_of_elements in physHistPersLook. *)
+(*         eapply elem_of_not_nil. *)
+(*         done. *)
+(*       } *)
+
+(*       assert (is_Some $ absHist !! t_full) as [full_encS absHistFullLook]. { *)
+(*         apply elem_of_dom. *)
+(*         rewrite /max_msg. *)
+(*         apply elem_of_elements. *)
+(*         rewrite -physEncDomEq. *)
+(*         apply max_list_elem_of. *)
+(*         apply elem_of_dom_2 in physHistPersLook. *)
+(*         apply elem_of_elements in physHistPersLook. *)
+(*         eapply elem_of_not_nil. *)
+(*         done. *)
+(*       } *)
+
+(*       (* lookup for read states (at crash timestamp) *) *)
+(*       assert (is_Some $ physHist !! (tCrash)) as [read_msg physHistReadLook]. { *)
+(*         rewrite /tCrash -Nat.add_comm. *)
+(*         rewrite -drop_prefix_lookup. *)
+(*         eapply valid_slice_lookup; [ exact cvSlicesPhysHists | done | ]. *)
+(*         apply map_lookup_zip_with_Some. *)
+(*         by exists physHist, oldOffset. *)
+(*       } *)
+
+(*       assert (is_Some $ absHist !! (tCrash)) as [crash_encS absHistCrashLook]. { *)
+(*         rewrite /tCrash -Nat.add_comm. *)
+(*         rewrite -drop_prefix_lookup. *)
+(*         rewrite -valid_slice_drop_prefix in cvSlicesAbsHists. *)
+(*         eapply valid_slice_lookup; [ exact cvSlicesAbsHists | done | ]. *)
+(*         apply map_lookup_zip_with_Some. *)
+(*         by exists absHist, oldOffset. *)
+(*       } *)
+
+(*       (* We try to allocate all the predicates for the next generation *) *)
+(* (*        * first, all [read] predicates except for the [tCrash] predicate are still *) *)
+(* (*        * allocated [read]. *) *)
+(* (*        * second, the pers predicate, the read predicate at [tCrash], and one of the *) *)
+(* (*        * full predicate after [tCrash] are allocated for the full recovery *) *)
+(* (*        * third, all full predicates before [tCrash] are reduced to [read] predicates *) *)
+(* (*        * for the next generation. *) *)
+(* (*        * *) *)
+
+(*       (* The crash timestamp is special for read predicates *) *)
+(*       iPoseProof (big_sepM2_delete with "readEncs") as "[readEncAtCrash readEncs]"; *)
+(*         [ eassumption | done | ]. *)
+(*       iPoseProof ((big_sepM2_split (λ t _ _, tCrash ≤ t)) with "fullEncs") *)
+(*         as "[fullAfterCrash fullBeforeCrash]". *)
+
+(*       rewrite [(▷ _ ∗ ▷ _ ∗ _)%I]bi.sep_assoc. *)
+(*       iApply (wand_passthrough with "[] [] [baseMap pcRes] [persEnc fullAfterCrash readEncAtCrash] [readEncs fullBeforeCrash]"); *)
+(*         [ | | iAccu | iAccu | iAccu ]. *)
+(*       { (* proof for full and pers *) *)
+(*         iIntros "((persEnc & fullEncs & readEncAtCrash) & baseMap & pcRes)". *)
+(*         iPoseProof ((big_sepM2_delete _ _ _ tCrash) with "fullEncs") as "[fullEncAtCrash fullEncs]"; *)
+(*           [ done | done | ]. *)
+(*         iSpecialize ("fullEncAtCrash" with "[//]"). *)
+(*         iDestruct (big_sepM2_lookup with "predFullPostCrash") *)
+(*           as (pred_read' pred_pers' order) "(% & % & %orderLook & postCrash)"; *)
+(*           [ apply predsFullLook | apply bumpersLook | ]. *)
+(*         rewrite drop_above_lookup_t in newMsgLook. *)
+(*         rewrite lookup_omap drop_above_lookup_t absHistCrashLook in H0. *)
+(*         simplify_eq. *)
+(*         (* case distinction on whether we crashed at the full timestamp *) *)
+(*         destruct (Nat.eq_dec t_full (tCrash)) as [ Heq | ? ]. *)
+(*         - (* we crash at [t_full] *) *)
+(*           iClear "readEncAtCrash fullEncs". *)
+(*           (* lookup for full predicate *) *)
+(*           simplify_eq. *)
+(*           iSpecialize ("fullEncAtCrash" with "[%] [%]"); *)
+(*             [ lia | by rewrite -Nat.add_1_r -Heq lookup_max_msg_succ | ]. *)
+(*           rewrite -> Heq in *. *)
+(*           simplify_eq. *)
+(*           (* we will use the join view for [predPostCrash] *) *)
+(*           set V_pers := (v in encoded_predicate_holds _ old_pers_encS _ (v, _)). *)
+(*           set V_full := (v in encoded_predicate_holds _ full_encS _ (v, _)). *)
+(*           pose proof (thread_view_le_l V_pers V_full). *)
+(*           assert ((V_pers, hGD) ⊑ (V_pers ⊔ V_full, hGD)) by (split; [ apply thread_view_le_l | done ]). *)
+(*           rewrite [encoded_predicate_holds _ _ _ (V_pers, _)]encoded_predicate_holds_mono; last done. *)
+(*           assert ((V_full, hGD) ⊑ (V_pers ⊔ V_full, hGD)) by (split; [ apply thread_view_le_r | done ]). *)
+(*           rewrite [encoded_predicate_holds _ _ _ (V_full, _)]encoded_predicate_holds_mono; last done. *)
+(*           iSpecialize ("postCrash" $! old_pers_encS old_pers_msg.(msg_val) *)
+(*                         with "[$persEnc]"). *)
+(*           iDestruct "postCrash" as "[postCrash _]". *)
+(*           iSpecialize ("postCrash" $! full_encS _ full_msg.(msg_val) with "fullEncAtCrash"). *)
+(*           iDestruct ("postCrash" with "[//]") as (P_full P_pers) "(#fullEq & #persEq & pred)". *)
+(*           iSimpl in "pred". *)
+(*           iDestruct ("pred" $! _ _ bumpers na_views store _ *)
+(*                       with "persImpl baseMap") as "(baseMap & pred)". *)
+(*           iDestruct ("pred" with "[$pcResPers $pcRes]") as "[H pcRes]". *)
+(*           iFrame. *)
+(*           setoid_rewrite <- bi.later_exist_2. *)
+(*           rewrite bi.sep_exist_r. *)
+(*           iExists _. *)
+(*           distrib_later. *)
+(*           pull_left (▷ (_ ≡ Some _))%I. *)
+(*           iSplit; first done. *)
+(*           pull_left (∃ _, _)%I. *)
+(*           rewrite bi.sep_exist_r. *)
+(*           iExists _. *)
+(*           distrib_later. *)
+(*           pull_left (▷ (_ ≡ Some _))%I. *)
+(*           iSplit; first done. *)
+(*           iFrame. *)
+(*           rewrite -bi.later_sep. *)
+(*           rewrite [(P_pers _ ∗ _)%I] bi.sep_comm. *)
+(*           iNext. *)
+(*           iSpecialize ("H" $! CV). *)
+(*           rewrite monPred_wand_force. *)
+(*           monPred_simpl. *)
+(*           iApply "H". *)
+(*           iSimpl. *)
+(*           iFrame "newCrashedAt". *)
+(*           assert (msg_persisted_after_view full_msg ⊑ CV). { *)
+(*             eapply consistent_cut_extract; [done | done | | |  ]. *)
+(*             - eapply lookup_weaken; last done. *)
+(*               apply map_lookup_zip_with_Some. *)
+(*               eexists _, _. split_and!; done. *)
+(*             - apply drop_prefix_lookup_Some_2. *)
+(*               rewrite Nat.add_comm. *)
+(*               done. *)
+(*             - lia. *)
+(*           } *)
+(*           assert (msg_persisted_after_view old_pers_msg ⊑ CV). { *)
+(*             destruct globalPViewLook as [globalPViewLook | [? ?]]. *)
+(*             - rewrite map_lookup_zip_with_Some in globalPViewLook. *)
+(*               destruct globalPViewLook as (? & [?] & ? & ? & globalPViewLook). *)
+(*               simplify_eq. *)
+(*               eapply consistent_cut_extract; [done | done | | |  ]. *)
+(*               + eapply lookup_weaken; last done. *)
+(*                 apply map_lookup_zip_with_Some. *)
+(*                 eexists _, _. split_and!; done. *)
+(*               + apply drop_prefix_lookup_Some_2. *)
+(*                 rewrite Nat.add_comm. *)
+(*                 done. *)
+(*               + assert (global_pview ≼ CV) as view_included by (by etrans). *)
+(*                 rewrite lookup_included in view_included. *)
+(*                 rewrite -Some_MaxNat_included -cvLook -globalPViewLook. *)
+(*                 done. *)
+(*             - eapply consistent_cut_extract; [done | done | | |  ]. *)
+(*               + eapply lookup_weaken; last done. *)
+(*                 apply map_lookup_zip_with_Some. *)
+(*                 eexists _, _. split_and!; done. *)
+(*               + apply drop_prefix_lookup_Some_2. *)
+(*                 rewrite Nat.add_comm. *)
+(*                 rewrite [old_ts]plus_n_O in physHistPersLook. *)
+(*                 done. *)
+(*               + lia. *)
+(*           } *)
+(*           iSplitPure; first by apply view_lub_le. *)
+(*           iApply (persisted_weak with "pers"). *)
+(*           f_equiv. *)
+(*           by apply view_lub_le. *)
+(*         - (* we crash at some other timestamps, we should use the second rule *) *)
+(*           (* but first, we need to sort out the proper thread view *) *)
+(*           iPoseProof (big_sepM2_lookup with "fullEncs [%] [%] [%]") as "fullEnc"; *)
+(*             do ? (rewrite lookup_delete_ne; last done); *)
+(*             [ apply physHistFullLook | *)
+(*               apply absHistFullLook | | | *)
+(*               by rewrite -Nat.add_1_r lookup_max_msg_succ | ]. *)
+(*             { apply max_list_elem_of_le. *)
+(*               rewrite elem_of_elements elem_of_dom. *)
+(*               by eexists. } *)
+(*             { apply (Nat.le_trans _ old_ts). *)
+(*               - destruct globalPViewLook as [globalPViewLook | []]. *)
+(*                 + rewrite map_lookup_zip_with_Some in globalPViewLook. *)
+(*                   destruct globalPViewLook as (x & [] & ? & ? & ?). *)
+(*                   simplify_eq. *)
+(*                   lia. *)
+(*                 + simplify_eq. *)
+(*                   lia. *)
+(*               - apply max_list_elem_of_le. *)
+(*                 apply elem_of_elements. *)
+(*                 apply elem_of_dom. *)
+(*                 by exists old_pers_msg. } *)
+(*           set V_pers := (v in encoded_predicate_holds _ old_pers_encS _ (v, _)). *)
+(*           set V_read := (v in encoded_predicate_holds _ crash_encS _ (v, _)). *)
+(*           iAssert (encoded_predicate_holds predRead crash_encS (msg_val read_msg) (V_read, hGD))%I *)
+(*             with "[readEncAtCrash fullEncAtCrash]" as "readEnc". { *)
+(*             assert (oldOffset ≤ tCrash) by lia. *)
+(*             destruct (physHist !! S tCrash). *)
+(*             - iApply "readEncAtCrash". *)
+(*               iPureIntro; right; done. *)
+(*             - iDestruct (big_sepM2_lookup with "predFullReadSplit") as "#split"; [ done | done | ]. *)
+(*               iSpecialize ("fullEncAtCrash" with "[%] [//]"); first lia. *)
+(*               iApply "split". *)
+(*               iFrame. *)
+(*           } *)
+(*           assert ((V_pers, hGD) ⊑ (V_pers ⊔ V_read, hGD)) by (split; [ apply thread_view_le_l | done ]). *)
+(*           rewrite [encoded_predicate_holds _ _ _ (V_pers, _)]encoded_predicate_holds_mono; last done. *)
+(*           assert ((V_read, hGD) ⊑ (V_pers ⊔ V_read, hGD)) by (split; [ apply thread_view_le_r | done ]). *)
+(*           rewrite [encoded_predicate_holds _ _ _ (V_read, _)]encoded_predicate_holds_mono; last done. *)
+(*           iSpecialize ("postCrash" $! old_pers_encS old_pers_msg.(msg_val) with "[$persEnc]"). *)
+(*           iDestruct "postCrash" as "[_ postCrash]". *)
+(*           iDestruct (big_sepM2_lookup with "ordered") as "%ordered"; [ done | done | ]. *)
+(*           iDestruct "fullEnc" as (P_full) "[#eqPFull PFullHolds]". *)
+(*           iDestruct ("postCrash" $! full_encS crash_encS new_encS full_msg.(msg_val) read_msg.(msg_val) P_full *)
+(*                         with "[$]") as (P_obj) "[PFullImplObj postCrash]". *)
+(*           rewrite monPred_at_objectively. *)
+(*           iSpecialize ("PFullImplObj" with "PFullHolds"). *)
+(*           rewrite monPred_at_objectively. *)
+(*           iSpecialize ("PFullImplObj" $! (V_pers ⊔ V_read, hGD)). *)
+(*           iDestruct ("postCrash" with "[$PFullImplObj] [//] [%] [%] [$readEnc]") *)
+(*             as (P_full' P_pers') "(#eqFull & #eqPers & pred)". *)
+(*           { assert (old_ts ≤ tCrash). { *)
+(*               rewrite map_lookup_zip_with_Some in globalPViewLook. *)
+(*               destruct globalPViewLook as [globalPViewLook | []]. *)
+(*               - destruct globalPViewLook as (? & [?] & ? & ? & globalPViewLook). *)
+(*                 simplify_eq. *)
+(*                 apply plus_le_compat_l. *)
+(*                 rewrite -Some_MaxNat_included -cvLook -globalPViewLook. *)
+(*                 assert (global_pview ≼ CV) as view_included by (by etrans). *)
+(*                 rewrite lookup_included in view_included. *)
+(*                 done. *)
+(*               - simplify_eq. *)
+(*                 lia. *)
+(*             } *)
+(*             destruct (Nat.eq_dec old_ts tCrash); [simplify_eq; by right | left]. *)
+(*             eapply ordered; [ | done | done ]. *)
+(*             lia. } *)
+(*           { assert (tCrash ≤ t_full). { *)
+(*               apply max_list_elem_of_le. *)
+(*               rewrite elem_of_elements elem_of_dom. *)
+(*               by eexists. *)
+(*             } *)
+(*             eapply ordered; [ | done | done ]. *)
+(*             lia. } *)
+(*           iEval (simpl) in "pred". *)
+(*           iDestruct ("pred" $! _ _ bumpers na_views store _ *)
+(*                       with "persImpl baseMap") as "(baseMap & pred)". *)
+(*           iDestruct ("pred" with "[$pcResPers $pcRes]") as "[H pcRes]". *)
+(*           iFrame. *)
+(*           setoid_rewrite <- bi.later_exist_2. *)
+(*           rewrite bi.sep_exist_r. *)
+(*           iExists _. *)
+(*           distrib_later. *)
+(*           pull_left (▷ (_ ≡ Some _))%I. *)
+(*           iSplit; first done. *)
+(*           pull_left (∃ _, _)%I. *)
+(*           rewrite bi.sep_exist_r. *)
+(*           iExists _. *)
+(*           distrib_later. *)
+(*           pull_left (▷ (_ ≡ Some _))%I. *)
+(*           iSplit; first done. *)
+(*           iFrame. *)
+(*           rewrite -bi.later_sep. *)
+(*           rewrite [(P_pers' _ ∗ _)%I] bi.sep_comm. *)
+(*           iNext. *)
+(*           iSpecialize ("H" $! CV). *)
+(*           rewrite monPred_wand_force. *)
+(*           monPred_simpl. *)
+(*           iApply "H". *)
+(*           iSimpl. *)
+(*           iFrame "newCrashedAt". *)
+(*           assert (msg_persisted_after_view read_msg ⊑ CV). { *)
+(*             eapply consistent_cut_extract; [done | done | | |  ]. *)
+(*             - eapply lookup_weaken; last done. *)
+(*               apply map_lookup_zip_with_Some. *)
+(*               eexists _, _. split_and!; done. *)
+(*             - apply drop_prefix_lookup_Some_2. *)
+(*               rewrite Nat.add_comm. *)
+(*               done. *)
+(*             - lia. *)
+(*           } *)
+(*           assert (msg_persisted_after_view old_pers_msg ⊑ CV). { *)
+(*             rewrite map_lookup_zip_with_Some in globalPViewLook. *)
+(*             destruct globalPViewLook as [globalPViewLook | []]. *)
+(*             - destruct globalPViewLook as (? & [] & ? & ? & GlobalPViewLook). *)
+(*               simplify_eq. *)
+(*               eapply consistent_cut_extract; [done | done | | |  ]. *)
+(*               + eapply lookup_weaken; last done. *)
+(*                 apply map_lookup_zip_with_Some. *)
+(*                 eexists _, _. split_and!; done. *)
+(*               + apply drop_prefix_lookup_Some_2. *)
+(*                 rewrite Nat.add_comm. *)
+(*                 done. *)
+(*               + assert (global_pview ≼ CV) as view_included by (by etrans). *)
+(*                 rewrite lookup_included in view_included. *)
+(*                 rewrite -Some_MaxNat_included -cvLook -GlobalPViewLook. *)
+(*                 done. *)
+(*             - eapply consistent_cut_extract; [done | done | | |  ]. *)
+(*               + eapply lookup_weaken; last done. *)
+(*                 apply map_lookup_zip_with_Some. *)
+(*                 eexists _, _. split_and!; done. *)
+(*               + apply drop_prefix_lookup_Some_2. *)
+(*                 rewrite Nat.add_comm. *)
+(*                 rewrite [old_ts]plus_n_O in physHistPersLook. *)
+(*                 done. *)
+(*               + lia. *)
+(*           } *)
+(*           iSplitPure; first by apply view_lub_le. *)
+(*           iApply (persisted_weak with "pers"). *)
+(*           f_equiv. *)
+(*           by apply view_lub_le. *)
+(*       } *)
+(*       { *)
+(*         iIntros "([readEncs fullEncs] & baseMap & pcRes)". *)
+(*         rewrite [([∗ map] _ ↦ _; _ ∈ _; _, ▷ _)%I](big_sepM2_delete _ _ _ tCrash); *)
+(*         [ | rewrite lookup_fmap_Some; by eexists | done ]. *)
+(*         rewrite [(discard_msg_views <$> _) !! _]lookup_fmap drop_above_lookup_gt; last lia. *)
+(*         pull_left (▷ _)%I. *)
+(*         iSplitL "". { *)
+(*           iIntros "!>" (Hcontra). *)
+(*           destruct Hcontra as [ | Hcontra ]; [ lia | by apply is_Some_None in Hcontra ]. *)
+(*         } *)
+(*         pull_right ([∗ map] _ ↦ _; _ ∈ _; _, _)%I. *)
+
+(*         (* merge full predicates and read predicates into one single [∗ map] for *) *)
+(* (*          * the next lemma. *) *)
+(*         iPoseProof (big_sepM2_delete _ _ _ tCrash with "fullEncs") as "[_ fullEncs]"; *)
+(*           [ done | done | ]. *)
+(*         iPoseProof (big_sepM2_sep_2 with "readEncs fullEncs") as "encs". *)
+
+(*         iApply (big_sepM2_impl_dom_subseteq_with_resource with "[baseMap pcRes] encs"). *)
+(*         { *)
+(*           rewrite 2!dom_delete. *)
+(*           rewrite dom_fmap_L. *)
+(*           apply difference_mono_r. *)
+(*           apply dom_filter_subseteq. *)
+(*         } *)
+(*         { *)
+(*           rewrite 2!dom_delete_L. *)
+(*           rewrite dom_fmap_L. *)
+(*           erewrite drop_above_dom_eq; last apply physEncDomEq. *)
+(*           rewrite dom_omap_id_L; first done. *)
+(*           eapply map_Forall_subseteq; last apply map. *)
+(*           apply map_filter_subseteq. *)
+(*         } *)
+(*         { iFrame. } *)
+(*         iIntros "!>" (t msg oldS ? newS physHistLook absHistLook). *)
+(*         assert (tCrash ≠ t) by (by apply lookup_delete_Some in physHistLook as [? _]). *)
+(*         rewrite ?(lookup_delete_ne _ tCrash t ltac:(done)). *)
+(*         rewrite lookup_delete_ne in physHistLook; last done. *)
+(*         rewrite lookup_delete_ne in absHistLook; last done. *)
+(*         iIntros ((? & <- & look)%lookup_fmap_Some bumperLook). *)
+(*         apply map_filter_lookup_Some in look as [??]. *)
+(*         apply lookup_omap_Some in bumperLook as (? & ? & (? & ?)%map_filter_lookup_Some). *)
+(*         simplify_eq. *)
+(*         iIntros "[baseMap pcRes] [predReadHolds predFullHolds]". *)
+(*         iSpecialize ("predFullHolds" with "[%]"); first lia. *)
+(*         pull_left (▷ _)%I. *)
+(*         iAssert (encoded_predicate_holds predRead oldS (msg_val msg) *)
+(*                    (default (msg_store_view msg) (na_views !! ℓ), *)
+(*                       msg_persisted_after_view msg, ∅, hGD))%I *)
+(*           with "[predReadHolds predFullHolds]" as "predReadHolds". { *)
+(*           destruct (decide (oldOffset ≤ t ∧ physHist !! S t = None)) as [ [] | yes ]. *)
+(*           - iSpecialize ("predFullHolds" with "[//] [//]"). *)
+(*             iPoseProof (big_sepM2_lookup with "predFullReadSplit predFullHolds") as "split"; *)
+(*               [ done | done | ]. *)
+(*             iFrame. *)
+(*           - iApply ("predReadHolds" with "[%]"). *)
+(*             apply not_and_l in yes as [ | ]. *)
+(*             + left. lia. *)
+(*             + right. by destruct (physHist !! S t) eqn:Heqn. *)
+(*         } *)
+(*         (* It's time to lookup the postcrash invariant *) *)
+(*         iDestruct (big_sepM2_lookup with "predReadPostCrash [//] [$predReadHolds]") *)
+(*           as (?P) "[#predEq pred]"; [apply predsReadLook | apply bumpersLook | ]. *)
+(*         iEval (simpl) in "pred". *)
+(*         iDestruct ("pred" $! _ _ bumpers na_views store _ *)
+(*                     with "persImpl baseMap") as "(baseMap & pred)". *)
+(*         iDestruct ("pred" with "[$pcResPers $pcRes]") as "[H pcRes]". *)
+(*         iFrame. *)
+(*         iIntros "!>" (_). *)
+(*         iExists _. *)
+(*         iFrame "#". *)
+(*         iEval (simpl). *)
+(*         assert (default ∅ (newNaViews !! ℓ) = ∅) as ->. { *)
+(*           rewrite /newNaViews. *)
+(*           destruct (gset_to_gmap ∅ newNaLocs !! ℓ) eqn:eq. *)
+(*           - apply lookup_gset_to_gmap_Some in eq as [_ ->]. done. *)
+(*           - done. *)
+(*         } *)
+(*         iApply ("H" $! CV). *)
+(*         iSimpl. *)
+(*         iFrame "newCrashedAt". *)
+(*         iDestruct (big_sepM2_lookup with "oldViewsDiscarded") as %disc; [done | done | ]. *)
+(*         assert (msg_persisted_after_view msg ⊑ CV). { *)
+(*           assert (t < oldOffset ∨ oldOffset ≤ t) as [? | le] by lia. *)
+(*           { eassert _ as eq by (by eapply disc). *)
+(*             rewrite -eq. *)
+(*             apply view_empty_least. } *)
+(*           apply Nat.le_exists_sub in le as (tt & eq & ?). *)
+(*           eapply consistent_cut_extract; [done | done | | |  ]. *)
+(*           - eapply lookup_weaken; last done. *)
+(*             apply map_lookup_zip_with_Some. *)
+(*             eexists _, _. split_and!; done. *)
+(*           - apply drop_prefix_lookup_Some_2. *)
+(*             erewrite <- eq. *)
+(*             done. *)
+(*           - lia. *)
+(*         } *)
+(*         iSplitPure; first done. *)
+(*         iApply (persisted_weak with "pers"). *)
+(*         f_equiv. *)
+(*         done. *)
+(*       } *)
+(*     } *)
+(*     (* [bumpMono] - Show that the bumpers are still monotone. *) *)
+(*     iSplitR "". *)
+(*     { iApply (big_sepM2_impl_subseteq with "bumpMono"). *)
+(*       { apply restrict_subseteq. } *)
+(*       { apply restrict_subseteq. } *)
+(*       { rewrite /newOrders /newBumpers. *)
+(*         rewrite 2!restrict_dom_L. *)
+(*         rewrite -domOrdersEqBumpers. *)
+(*         done. } } *)
+(*     (* domain equations *) *)
+(*     do 3 (iSplitPure; first (rewrite 2!restrict_dom_L; congruence)). *)
+
+(*     (* [predPostCrash] - a little bit more complicated due to we look up more than two maps now *) *)
+(*     iSplitR "". { *)
+(*       iApply big_sepM2_impl. { *)
+(*         iApply (big_sepM2_impl_subseteq with "predFullPostCrash"). *)
+(*         { by apply restrict_subseteq. } *)
+(*         { by apply restrict_subseteq. } *)
+(*         { rewrite 2!restrict_dom_L. *)
+(*           rewrite -FullBumperDoms. *)
+(*           done. } *)
+(*       } *)
+(*       { iIntros "!> !>" (ℓ predFull bumper) "%predFullLook %bumperLook *)
+(*         (%predRead & %predPers & %order & %predReadLook & %predPersLook & %orderLook & ?)". *)
+(*         iExists predRead, predPers, order. *)
+(*         assert (ℓ ∈ recLocs). { *)
+(*           rewrite restrict_lookup_Some in predFullLook. *)
+(*           tauto. *)
+(*         } *)
+(*         do 3 (iSplitPure; first by rewrite restrict_lookup_elem_of). *)
+(*         iFrame. *)
+(*       } *)
+(*     } *)
+
+(*     (* [predReadPostCrash] *) *)
+(*     iSplitR "". { *)
+(*       iApply (big_sepM2_impl_subseteq with "predReadPostCrash"). *)
+(*       { by apply restrict_subseteq. } *)
+(*       { by apply restrict_subseteq. } *)
+(*       { rewrite 2!restrict_dom_L. *)
+(*         rewrite -ReadBumperDoms. *)
+(*         done. } *)
+(*     } *)
+(*     (* [predFullReadSplit] *) *)
+(*     iSplitR "". { *)
+(*       iApply (big_sepM2_impl_subseteq with "predFullReadSplit"). *)
+(*       { by apply restrict_subseteq. } *)
+(*       { by apply restrict_subseteq. } *)
+(*       { rewrite 2!restrict_dom_L. *)
+(*         rewrite ReadBumperDoms FullBumperDoms. *)
+(*         done. } *)
+(*     } *)
+(*     (* bumperBumpToValid *) *)
+(*     iSplitPure. *)
+(*     { eapply map_Forall_subseteq; last done. *)
+(*       apply restrict_subseteq. } *)
+(*     (* bumperSome *) *)
+(*     { iApply big_sepM2_forall. *)
+(*       iSplitPure. *)
+(*       { apply dom_eq_alt_L. *)
+(*         rewrite restrict_dom_subset_L; first done. *)
+(*         rewrite /recLocs. *)
+(*         rewrite domHistsEqBumpers. *)
+(*         set_solver+. } *)
+(*       iIntros (ℓ hist bumper look look2). *)
+(*       apply new_abs_hist_lookup_Some in look. *)
+(*       destruct look as (bumper' & s & ? & hist' & ? & ? & ?). *)
+(*       simplify_eq. *)
+(*       assert (bumper = bumper') as <-. *)
+(*       { eapply lookup_weaken_inv; [done| |done]. apply restrict_subseteq. } *)
+(*       iNext. iIntros (?? look). *)
+(*       iDestruct (big_sepM2_lookup with "bumperSome") as %i; [done|done|]. *)
+(*       apply lookup_omap_Some in look as (? & ? & (? & ?)%map_filter_lookup_Some). *)
+(*       eapply map_Forall_lookup_1 in i as [bumpedS eq]; last done. *)
+(*       simplify_eq. *)
+(*       eapply map_Forall_lookup_1 in bumperBumpToValid as [spa equi]; last done; first done. *)
+(*       rewrite equi. *)
+(*       done. } *)
+  Admitted.
 
   (* _The_ lemma for showing a recovery weakest precondition. *)
-  Lemma idempotence_wpr s E1 e rec Φ Φr (Φc : dProp Σ) `{!ViewObjective Φc} :
+  Lemma idempotence_wpr `{!nvmBaseG Σ Ω, !nvmHighG Σ Ω, !PerennialG Σ} s E1 e rec Φ Φr (Φc : dProp Σ) `{!Objective Φc} :
     ⊢ WPC e @ s ; E1 {{ Φ }} {{ Φc }} -∗
-      (<obj> □ (Φc -∗ post_crash (WPC rec @ s ; E1 {{ Φr }} {{ Φc }}))) -∗
+      (<obj> ■ (Φc -∗ <NG> (WPC rec @ s ; E1 {{ Φr }} {{ Φc }}))) -∗
       wpr s E1 e rec Φ Φr.
   Proof.
     iModel.
-    iLöb as "IH" forall (e Φ gnames TV).
-
+    iRevert (e Φ TV).
+    iApply löb_wand_plainly.
+    iIntros "!> #IH" (e Φ TV).
     monPred_simpl.
     iIntros "wpc".
-    introsIndex ? ?.
-    iIntros "#Hidemp".
-    rewrite /wpr.
-    rewrite wpr_unfold.
-    rewrite /wpr_pre.
-    assert ((TV, gnames) ⊑ (p, gnames)). { split; last done. solve_view_le. }
-    iApply (wpc_strong_mono' with  "wpc"); try reflexivity.
+    iIntros (TV' ?) "#Hidemp".
+    iIntros .
+    rewrite /wpr wpr_unfold /wpr_pre.
+    iApply (wpc_strong_mono' with "wpc"); [ by auto | by auto | ].
     iSplit. { iIntros (?). monPred_simpl. setoid_rewrite monPred_at_fupd. auto. }
     monPred_simpl.
-    introsIndex ? ?.
-    iIntros "phiC".
+    iIntros (TV'' ?) "Φc".
     iModIntro.
-    iIntros (???? step ns ?).
-    iDestruct ("Hidemp" with "phiC") as "idemp'".
-    rewrite lift_d_at.
-    iIntros "state global".
-    iIntros (γcrash ?) "NC".
-    (* Allocate the new ghost state. *)
-    iMod (nvm_reinit _ _ _ _ _ _ _ γcrash with "state idemp'")
-      as (names) "(%crEq & val & stateInterp & HIHI & idemp)".
-    { apply step. }
-    iDestruct "global" as "($ & Hc & $ & $)".
-    assert (exists k, ns + k = step_count_next ns) as [k' eq].
-    { eexists _. rewrite /step_count_next. simpl. rewrite -assoc. reflexivity. }
-    iMod (cred_frag.cred_interp_incr_k _ k' with "Hc") as "(Hc & _)".
-    rewrite eq.
+    iIntros (???? step ns ?) "state global".
+    iMod (nvm_reinit with "state") as "state"; first done.
+    iModIntro.
+    iDestruct ("Hidemp" with "Φc") as "Hidemp'".
+    iEval (rewrite /high.modalities.nextgen.nextgen /=) in "Hidemp'".
+    iModIntro.
+    iMod "state" as "(#validV & interp & nvm_heap_ctx)".
+    iModIntro.
+    rewrite /state_interp /=.
+    iFrame "∗#".
 
-    iModIntro (|={E1}=> _)%I.
-    iExists names.
-    iSplit; first done.
-    simpl.
-    rewrite /get_crash_name in crEq. rewrite -crEq.
-    iFrame "NC".
-    iFrame.
-    monPred_simpl.
-    iSpecialize ("IH" $! _ _ names with "idemp [Hidemp]").
+    iSplitL "". { rewrite /global_state_interp /=. admit. } (* global state interp a.k.a. crash borrows *)
+
+    iModIntro.
+    iSpecialize ("IH" $! _ _ with "Hidemp' [Hidemp]").
     { monPred_simpl. done. }
     iApply "IH".
-  Qed.
+  Admitted.
 
 End wpr.
